src/HOL/UNITY/Comp.thy
@@ -9,7 +9,7 @@ Technical Report 2000-003, University of Florida, 2000.
 
 Revised by Sidi Ehmety on January  2001 
 
-Added: a strong form of the <= relation (component_of) and localize 
+Added: a strong form of the \<subseteq> relation (component_of) and localize 
 
 *)
 
@@ -20,33 +20,32 @@ theory Comp = Union:
 instance program :: (type) ord ..
 
 defs
-  component_def:          "F <= H == EX G. F Join G = H"
-  strict_component_def:   "(F < (H::'a program)) == (F <= H & F ~= H)"
+  component_def:          "F \<le> H == \<exists>G. F Join G = H"
+  strict_component_def:   "(F < (H::'a program)) == (F \<le> H & F \<noteq> H)"
 
 
 constdefs
-  component_of :: "'a program=>'a program=> bool"
+  component_of :: "'a program =>'a program=> bool"
                                     (infixl "component'_of" 50)
-  "F component_of H == EX G. F ok G & F Join G = H"
+  "F component_of H == \<exists>G. F ok G & F Join G = H"
 
   strict_component_of :: "'a program\<Rightarrow>'a program=> bool"
                                     (infixl "strict'_component'_of" 50)
-  "F strict_component_of H == F component_of H & F~=H"
+  "F strict_component_of H == F component_of H & F\<noteq>H"
   
   preserves :: "('a=>'b) => 'a program set"
-    "preserves v == INT z. stable {s. v s = z}"
+    "preserves v == \<Inter>z. stable {s. v s = z}"
 
   localize  :: "('a=>'b) => 'a program => 'a program"
   "localize v F == mk_program(Init F, Acts F,
-			      AllowedActs F Int (UN G:preserves v. Acts G))"
+			      AllowedActs F \<inter> (\<Union>G \<in> preserves v. Acts G))"
 
   funPair      :: "['a => 'b, 'a => 'c, 'a] => 'b * 'c"
   "funPair f g == %x. (f x, g x)"
 
 
 subsection{*The component relation*}
-lemma componentI: 
-     "H <= F | H <= G ==> H <= (F Join G)"
+lemma componentI: "H \<le> F | H \<le> G ==> H \<le> (F Join G)"
 apply (unfold component_def, auto)
 apply (rule_tac x = "G Join Ga" in exI)
 apply (rule_tac [2] x = "G Join F" in exI)
@@ -54,61 +53,61 @@ apply (auto simp add: Join_ac)
 done
 
 lemma component_eq_subset: 
-     "(F <= G) =  
-      (Init G <= Init F & Acts F <= Acts G & AllowedActs G <= AllowedActs F)"
+     "(F \<le> G) =  
+      (Init G \<subseteq> Init F & Acts F \<subseteq> Acts G & AllowedActs G \<subseteq> AllowedActs F)"
 apply (unfold component_def)
 apply (force intro!: exI program_equalityI)
 done
 
-lemma component_SKIP [iff]: "SKIP <= F"
+lemma component_SKIP [iff]: "SKIP \<le> F"
 apply (unfold component_def)
 apply (force intro: Join_SKIP_left)
 done
 
-lemma component_refl [iff]: "F <= (F :: 'a program)"
+lemma component_refl [iff]: "F \<le> (F :: 'a program)"
 apply (unfold component_def)
 apply (blast intro: Join_SKIP_right)
 done
 
-lemma SKIP_minimal: "F <= SKIP ==> F = SKIP"
+lemma SKIP_minimal: "F \<le> SKIP ==> F = SKIP"
 by (auto intro!: program_equalityI simp add: component_eq_subset)
 
-lemma component_Join1: "F <= (F Join G)"
+lemma component_Join1: "F \<le> (F Join G)"
 by (unfold component_def, blast)
 
-lemma component_Join2: "G <= (F Join G)"
+lemma component_Join2: "G \<le> (F Join G)"
 apply (unfold component_def)
 apply (simp add: Join_commute, blast)
 done
 
-lemma Join_absorb1: "F<=G ==> F Join G = G"
+lemma Join_absorb1: "F \<le> G ==> F Join G = G"
 by (auto simp add: component_def Join_left_absorb)
 
-lemma Join_absorb2: "G<=F ==> F Join G = F"
+lemma Join_absorb2: "G \<le> F ==> F Join G = F"
 by (auto simp add: Join_ac component_def)
 
-lemma JN_component_iff: "((JOIN I F) <= H) = (ALL i: I. F i <= H)"
+lemma JN_component_iff: "((JOIN I F) \<le> H) = (\<forall>i \<in> I. F i \<le> H)"
 by (simp add: component_eq_subset, blast)
 
-lemma component_JN: "i : I ==> (F i) <= (JN i:I. (F i))"
+lemma component_JN: "i \<in> I ==> (F i) \<le> (\<Squnion>i \<in> I. (F i))"
 apply (unfold component_def)
 apply (blast intro: JN_absorb)
 done
 
-lemma component_trans: "[| F <= G; G <= H |] ==> F <= (H :: 'a program)"
+lemma component_trans: "[| F \<le> G; G \<le> H |] ==> F \<le> (H :: 'a program)"
 apply (unfold component_def)
 apply (blast intro: Join_assoc [symmetric])
 done
 
-lemma component_antisym: "[| F <= G; G <= F |] ==> F = (G :: 'a program)"
+lemma component_antisym: "[| F \<le> G; G \<le> F |] ==> F = (G :: 'a program)"
 apply (simp (no_asm_use) add: component_eq_subset)
 apply (blast intro!: program_equalityI)
 done
 
-lemma Join_component_iff: "((F Join G) <= H) = (F <= H & G <= H)"
+lemma Join_component_iff: "((F Join G) \<le> H) = (F \<le> H & G \<le> H)"
 by (simp add: component_eq_subset, blast)
 
-lemma component_constrains: "[| F <= G; G : A co B |] ==> F : A co B"
+lemma component_constrains: "[| F \<le> G; G \<in> A co B |] ==> F \<in> A co B"
 by (auto simp add: constrains_def component_eq_subset)
 
 (*Used in Guar.thy to show that programs are partially ordered*)
@@ -117,34 +116,34 @@ lemmas program_less_le = strict_component_def [THEN meta_eq_to_obj_eq]
 
 subsection{*The preserves property*}
 
-lemma preservesI: "(!!z. F : stable {s. v s = z}) ==> F : preserves v"
+lemma preservesI: "(!!z. F \<in> stable {s. v s = z}) ==> F \<in> preserves v"
 by (unfold preserves_def, blast)
 
 lemma preserves_imp_eq: 
-     "[| F : preserves v;  act : Acts F;  (s,s') : act |] ==> v s = v s'"
+     "[| F \<in> preserves v;  act \<in> Acts F;  (s,s') \<in> act |] ==> v s = v s'"
 apply (unfold preserves_def stable_def constrains_def, force)
 done
 
 lemma Join_preserves [iff]: 
-     "(F Join G : preserves v) = (F : preserves v & G : preserves v)"
+     "(F Join G \<in> preserves v) = (F \<in> preserves v & G \<in> preserves v)"
 apply (unfold preserves_def, auto)
 done
 
 lemma JN_preserves [iff]:
-     "(JOIN I F : preserves v) = (ALL i:I. F i : preserves v)"
+     "(JOIN I F \<in> preserves v) = (\<forall>i \<in> I. F i \<in> preserves v)"
 apply (simp add: JN_stable preserves_def, blast)
 done
 
-lemma SKIP_preserves [iff]: "SKIP : preserves v"
+lemma SKIP_preserves [iff]: "SKIP \<in> preserves v"
 by (auto simp add: preserves_def)
 
 lemma funPair_apply [simp]: "(funPair f g) x = (f x, g x)"
 by (simp add:  funPair_def)
 
-lemma preserves_funPair: "preserves (funPair v w) = preserves v Int preserves w"
+lemma preserves_funPair: "preserves (funPair v w) = preserves v \<inter> preserves w"
 by (auto simp add: preserves_def stable_def constrains_def, blast)
 
-(* (F : preserves (funPair v w)) = (F : preserves v Int preserves w) *)
+(* (F \<in> preserves (funPair v w)) = (F \<in> preserves v \<inter> preserves w) *)
 declare preserves_funPair [THEN eqset_imp_iff, iff]
 
 
@@ -157,20 +156,20 @@ by (simp add: funPair_def o_def)
 lemma snd_o_funPair [simp]: "snd o (funPair f g) = g"
 by (simp add: funPair_def o_def)
 
-lemma subset_preserves_o: "preserves v <= preserves (w o v)"
+lemma subset_preserves_o: "preserves v \<subseteq> preserves (w o v)"
 by (force simp add: preserves_def stable_def constrains_def)
 
-lemma preserves_subset_stable: "preserves v <= stable {s. P (v s)}"
+lemma preserves_subset_stable: "preserves v \<subseteq> stable {s. P (v s)}"
 apply (auto simp add: preserves_def stable_def constrains_def)
 apply (rename_tac s' s)
 apply (subgoal_tac "v s = v s'")
 apply (force+)
 done
 
-lemma preserves_subset_increasing: "preserves v <= increasing v"
+lemma preserves_subset_increasing: "preserves v \<subseteq> increasing v"
 by (auto simp add: preserves_subset_stable [THEN subsetD] increasing_def)
 
-lemma preserves_id_subset_stable: "preserves id <= stable A"
+lemma preserves_id_subset_stable: "preserves id \<subseteq> stable A"
 by (force simp add: preserves_def stable_def constrains_def)
 
 
@@ -183,27 +182,27 @@ by (auto intro: safety_prop_INTER1 simp add: preserves_def)
 (** Some lemmas used only in Client.ML **)
 
 lemma stable_localTo_stable2:
-     "[| F : stable {s. P (v s) (w s)};    
-         G : preserves v;  G : preserves w |]                
-      ==> F Join G : stable {s. P (v s) (w s)}"
-apply (simp (no_asm_simp))
-apply (subgoal_tac "G: preserves (funPair v w) ")
+     "[| F \<in> stable {s. P (v s) (w s)};    
+         G \<in> preserves v;  G \<in> preserves w |]                
+      ==> F Join G \<in> stable {s. P (v s) (w s)}"
+apply (simp)
+apply (subgoal_tac "G \<in> preserves (funPair v w) ")
  prefer 2 apply simp 
-apply (drule_tac P1 = "split ?Q" in  preserves_subset_stable [THEN subsetD], auto)
+apply (drule_tac P1 = "split ?Q" in preserves_subset_stable [THEN subsetD], auto)
 done
 
 lemma Increasing_preserves_Stable:
-     "[| F : stable {s. v s <= w s};  G : preserves v;        
-         F Join G : Increasing w |]                
-      ==> F Join G : Stable {s. v s <= w s}"
+     "[| F \<in> stable {s. v s \<le> w s};  G \<in> preserves v;        
+         F Join G \<in> Increasing w |]                
+      ==> F Join G \<in> Stable {s. v s \<le> w s}"
 apply (auto simp add: stable_def Stable_def Increasing_def Constrains_def all_conj_distrib)
 apply (blast intro: constrains_weaken)
 (*The G case remains*)
 apply (auto simp add: preserves_def stable_def constrains_def)
 apply (case_tac "act: Acts F", blast)
 (*We have a G-action, so delete assumptions about F-actions*)
-apply (erule_tac V = "ALL act:Acts F. ?P act" in thin_rl)
-apply (erule_tac V = "ALL z. ALL act:Acts F. ?P z act" in thin_rl)
+apply (erule_tac V = "\<forall>act \<in> Acts F. ?P act" in thin_rl)
+apply (erule_tac V = "\<forall>z. \<forall>act \<in> Acts F. ?P z act" in thin_rl)
 apply (subgoal_tac "v x = v xa")
 prefer 2 apply blast
 apply auto
@@ -212,12 +211,12 @@ done
 
 (** component_of **)
 
-(*  component_of is stronger than <= *)
-lemma component_of_imp_component: "F component_of H ==> F <= H"
+(*  component_of is stronger than \<le> *)
+lemma component_of_imp_component: "F component_of H ==> F \<le> H"
 by (unfold component_def component_of_def, blast)
 
 
-(* component_of satisfies many of the <='s properties *)
+(* component_of satisfies many of the same properties as \<le> *)
 lemma component_of_refl [simp]: "F component_of F"
 apply (unfold component_of_def)
 apply (rule_tac x = SKIP in exI, auto)
@@ -243,7 +242,7 @@ lemma localize_Acts_eq [simp]: "Acts (localize v F) = Acts F"
 by (simp add: localize_def)
 
 lemma localize_AllowedActs_eq [simp]: 
- "AllowedActs (localize v F) = AllowedActs F Int (UN G:(preserves v). Acts G)"
+ "AllowedActs (localize v F) = AllowedActs F \<inter> (\<Union>G \<in> preserves v. Acts G)"
 by (unfold localize_def, auto)
 
 end
