src/HOL/UNITY/Extend.thy
@@ -16,23 +16,23 @@ constdefs
 
   (*MOVE to Relation.thy?*)
   Restrict :: "[ 'a set, ('a*'b) set] => ('a*'b) set"
-    "Restrict A r == r Int (A <*> UNIV)"
+    "Restrict A r == r \<inter> (A <*> UNIV)"
 
   good_map :: "['a*'b => 'c] => bool"
-    "good_map h == surj h & (ALL x y. fst (inv h (h (x,y))) = x)"
+    "good_map h == surj h & (\<forall>x y. fst (inv h (h (x,y))) = x)"
      (*Using the locale constant "f", this is  f (h (x,y))) = x*)
   
   extend_set :: "['a*'b => 'c, 'a set] => 'c set"
     "extend_set h A == h ` (A <*> UNIV)"
 
   project_set :: "['a*'b => 'c, 'c set] => 'a set"
-    "project_set h C == {x. EX y. h(x,y) : C}"
+    "project_set h C == {x. \<exists>y. h(x,y) \<in> C}"
 
   extend_act :: "['a*'b => 'c, ('a*'a) set] => ('c*'c) set"
-    "extend_act h == %act. UN (s,s'): act. UN y. {(h(s,y), h(s',y))}"
+    "extend_act h == %act. \<Union>(s,s') \<in> act. \<Union>y. {(h(s,y), h(s',y))}"
 
   project_act :: "['a*'b => 'c, ('c*'c) set] => ('a*'a) set"
-    "project_act h act == {(x,x'). EX y y'. (h(x,y), h(x',y')) : act}"
+    "project_act h act == {(x,x'). \<exists>y y'. (h(x,y), h(x',y')) \<in> act}"
 
   extend :: "['a*'b => 'c, 'a program] => 'c program"
     "extend h F == mk_program (extend_set h (Init F),
@@ -56,7 +56,7 @@ locale Extend =
     good_h:  "good_map h"
   defines f_def: "f z == fst (inv h z)"
       and g_def: "g z == snd (inv h z)"
-      and slice_def: "slice Z y == {x. h(x,y) : Z}"
+      and slice_def: "slice Z y == {x. h(x,y) \<in> Z}"
 
 
 (** These we prove OUTSIDE the locale. **)
@@ -65,7 +65,7 @@ locale Extend =
 subsection{*Restrict*}
 (*MOVE to Relation.thy?*)
 
-lemma Restrict_iff [iff]: "((x,y): Restrict A r) = ((x,y): r & x: A)"
+lemma Restrict_iff [iff]: "((x,y): Restrict A r) = ((x,y): r & x \<in> A)"
 by (unfold Restrict_def, blast)
 
 lemma Restrict_UNIV [simp]: "Restrict UNIV = id"
@@ -76,29 +76,29 @@ done
 lemma Restrict_empty [simp]: "Restrict {} r = {}"
 by (auto simp add: Restrict_def)
 
-lemma Restrict_Int [simp]: "Restrict A (Restrict B r) = Restrict (A Int B) r"
+lemma Restrict_Int [simp]: "Restrict A (Restrict B r) = Restrict (A \<inter> B) r"
 by (unfold Restrict_def, blast)
 
-lemma Restrict_triv: "Domain r <= A ==> Restrict A r = r"
+lemma Restrict_triv: "Domain r \<subseteq> A ==> Restrict A r = r"
 by (unfold Restrict_def, auto)
 
-lemma Restrict_subset: "Restrict A r <= r"
+lemma Restrict_subset: "Restrict A r \<subseteq> r"
 by (unfold Restrict_def, auto)
 
 lemma Restrict_eq_mono: 
-     "[| A <= B;  Restrict B r = Restrict B s |]  
+     "[| A \<subseteq> B;  Restrict B r = Restrict B s |]  
       ==> Restrict A r = Restrict A s"
 by (unfold Restrict_def, blast)
 
 lemma Restrict_imageI: 
-     "[| s : RR;  Restrict A r = Restrict A s |]  
-      ==> Restrict A r : Restrict A ` RR"
+     "[| s \<in> RR;  Restrict A r = Restrict A s |]  
+      ==> Restrict A r \<in> Restrict A ` RR"
 by (unfold Restrict_def image_def, auto)
 
-lemma Domain_Restrict [simp]: "Domain (Restrict A r) = A Int Domain r"
+lemma Domain_Restrict [simp]: "Domain (Restrict A r) = A \<inter> Domain r"
 by blast
 
-lemma Image_Restrict [simp]: "(Restrict A r) `` B = r `` (A Int B)"
+lemma Image_Restrict [simp]: "(Restrict A r) `` B = r `` (A \<inter> B)"
 by blast
 
 lemma insert_Id_image_Acts: "f Id = Id ==> insert Id (f`Acts F) = f ` Acts F"
@@ -169,19 +169,19 @@ qed
 subsection{*@{term extend_set}: basic properties*}
 
 lemma project_set_iff [iff]:
-     "(x : project_set h C) = (EX y. h(x,y) : C)"
+     "(x \<in> project_set h C) = (\<exists>y. h(x,y) \<in> C)"
 by (simp add: project_set_def)
 
-lemma extend_set_mono: "A<=B ==> extend_set h A <= extend_set h B"
+lemma extend_set_mono: "A \<subseteq> B ==> extend_set h A \<subseteq> extend_set h B"
 by (unfold extend_set_def, blast)
 
-lemma (in Extend) mem_extend_set_iff [iff]: "z : extend_set h A = (f z : A)"
+lemma (in Extend) mem_extend_set_iff [iff]: "z \<in> extend_set h A = (f z \<in> A)"
 apply (unfold extend_set_def)
 apply (force intro: h_f_g_eq [symmetric])
 done
 
 lemma (in Extend) extend_set_strict_mono [iff]:
-     "(extend_set h A <= extend_set h B) = (A <= B)"
+     "(extend_set h A \<subseteq> extend_set h B) = (A \<subseteq> B)"
 by (unfold extend_set_def, force)
 
 lemma extend_set_empty [simp]: "extend_set h {} = {}"
@@ -198,7 +198,7 @@ lemma (in Extend) extend_set_inverse [simp]:
 by (unfold extend_set_def, auto)
 
 lemma (in Extend) extend_set_project_set:
-     "C <= extend_set h (project_set h C)"
+     "C \<subseteq> extend_set h (project_set h C)"
 apply (unfold extend_set_def)
 apply (auto simp add: split_extended_all, blast)
 done
@@ -220,7 +220,7 @@ lemma (in Extend) project_set_eq: "project_set h C = f ` C"
 by (auto intro: f_h_eq [symmetric] simp add: split_extended_all)
 
 (*Converse appears to fail*)
-lemma (in Extend) project_set_I: "!!z. z : C ==> f z : project_set h C"
+lemma (in Extend) project_set_I: "!!z. z \<in> C ==> f z \<in> project_set h C"
 by (auto simp add: split_extended_all)
 
 
@@ -228,31 +228,31 @@ subsection{*More laws*}
 
 (*Because A and B could differ on the "other" part of the state, 
    cannot generalize to 
-      project_set h (A Int B) = project_set h A Int project_set h B
+      project_set h (A \<inter> B) = project_set h A \<inter> project_set h B
 *)
 lemma (in Extend) project_set_extend_set_Int:
-     "project_set h ((extend_set h A) Int B) = A Int (project_set h B)"
+     "project_set h ((extend_set h A) \<inter> B) = A \<inter> (project_set h B)"
 by auto
 
 (*Unused, but interesting?*)
 lemma (in Extend) project_set_extend_set_Un:
-     "project_set h ((extend_set h A) Un B) = A Un (project_set h B)"
+     "project_set h ((extend_set h A) \<union> B) = A \<union> (project_set h B)"
 by auto
 
 lemma project_set_Int_subset:
-     "project_set h (A Int B) <= (project_set h A) Int (project_set h B)"
+     "project_set h (A \<inter> B) \<subseteq> (project_set h A) \<inter> (project_set h B)"
 by auto
 
 lemma (in Extend) extend_set_Un_distrib:
-     "extend_set h (A Un B) = extend_set h A Un extend_set h B"
+     "extend_set h (A \<union> B) = extend_set h A \<union> extend_set h B"
 by auto
 
 lemma (in Extend) extend_set_Int_distrib:
-     "extend_set h (A Int B) = extend_set h A Int extend_set h B"
+     "extend_set h (A \<inter> B) = extend_set h A \<inter> extend_set h B"
 by auto
 
 lemma (in Extend) extend_set_INT_distrib:
-     "extend_set h (INTER A B) = (INT x:A. extend_set h (B x))"
+     "extend_set h (INTER A B) = (\<Inter>x \<in> A. extend_set h (B x))"
 by auto
 
 lemma (in Extend) extend_set_Diff_distrib:
@@ -260,26 +260,26 @@ lemma (in Extend) extend_set_Diff_distrib:
 by auto
 
 lemma (in Extend) extend_set_Union:
-     "extend_set h (Union A) = (UN X:A. extend_set h X)"
+     "extend_set h (Union A) = (\<Union>X \<in> A. extend_set h X)"
 by blast
 
 lemma (in Extend) extend_set_subset_Compl_eq:
-     "(extend_set h A <= - extend_set h B) = (A <= - B)"
+     "(extend_set h A \<subseteq> - extend_set h B) = (A \<subseteq> - B)"
 by (unfold extend_set_def, auto)
 
 
 subsection{*@{term extend_act}*}
 
 (*Can't strengthen it to
-  ((h(s,y), h(s',y')) : extend_act h act) = ((s, s') : act & y=y')
+  ((h(s,y), h(s',y')) \<in> extend_act h act) = ((s, s') \<in> act & y=y')
   because h doesn't have to be injective in the 2nd argument*)
 lemma (in Extend) mem_extend_act_iff [iff]: 
-     "((h(s,y), h(s',y)) : extend_act h act) = ((s, s') : act)"
+     "((h(s,y), h(s',y)) \<in> extend_act h act) = ((s, s') \<in> act)"
 by (unfold extend_act_def, auto)
 
 (*Converse fails: (z,z') would include actions that changed the g-part*)
 lemma (in Extend) extend_act_D: 
-     "(z, z') : extend_act h act ==> (f z, f z') : act"
+     "(z, z') \<in> extend_act h act ==> (f z, f z') \<in> act"
 by (unfold extend_act_def, auto)
 
 lemma (in Extend) extend_act_inverse [simp]: 
@@ -292,7 +292,7 @@ lemma (in Extend) project_act_extend_act_restrict [simp]:
 by (unfold extend_act_def project_act_def, blast)
 
 lemma (in Extend) subset_extend_act_D: 
-     "act' <= extend_act h act ==> project_act h act' <= act"
+     "act' \<subseteq> extend_act h act ==> project_act h act' \<subseteq> act"
 by (unfold extend_act_def project_act_def, force)
 
 lemma (in Extend) inj_extend_act: "inj (extend_act h)"
@@ -305,7 +305,7 @@ lemma (in Extend) extend_act_Image [simp]:
 by (unfold extend_set_def extend_act_def, force)
 
 lemma (in Extend) extend_act_strict_mono [iff]:
-     "(extend_act h act' <= extend_act h act) = (act'<=act)"
+     "(extend_act h act' \<subseteq> extend_act h act) = (act'<=act)"
 by (unfold extend_act_def, auto)
 
 declare (in Extend) inj_extend_act [THEN inj_eq, iff]
@@ -322,7 +322,7 @@ apply (force intro: h_f_g_eq [symmetric])
 done
 
 lemma (in Extend) project_act_I: 
-     "!!z z'. (z, z') : act ==> (f z, f z') : project_act h act"
+     "!!z z'. (z, z') \<in> act ==> (f z, f z') \<in> project_act h act"
 apply (unfold project_act_def)
 apply (force simp add: split_extended_all)
 done
@@ -365,7 +365,7 @@ by (auto simp add: project_def image_iff)
 lemma (in Extend) AllowedActs_project [simp]:
      "AllowedActs(project h C F) =  
         {act. Restrict (project_set h C) act  
-               : project_act h ` Restrict C ` AllowedActs F}"
+               \<in> project_act h ` Restrict C ` AllowedActs F}"
 apply (simp (no_asm) add: project_def image_iff)
 apply (subst insert_absorb)
 apply (auto intro!: bexI [of _ Id] simp add: project_act_def)
@@ -386,14 +386,14 @@ lemma project_set_UNIV [simp]: "project_set h UNIV = UNIV"
 by auto
 
 lemma project_set_Union:
-     "project_set h (Union A) = (UN X:A. project_set h X)"
+     "project_set h (Union A) = (\<Union>X \<in> A. project_set h X)"
 by blast
 
 
 (*Converse FAILS: the extended state contributing to project_set h C
   may not coincide with the one contributing to project_act h act*)
 lemma (in Extend) project_act_Restrict_subset:
-     "project_act h (Restrict C act) <=  
+     "project_act h (Restrict C act) \<subseteq>  
       Restrict (project_set h C) (project_act h act)"
 by (auto simp add: project_act_def)
 
@@ -405,7 +405,7 @@ lemma (in Extend) project_extend_eq:
      "project h C (extend h F) =  
       mk_program (Init F, Restrict (project_set h C) ` Acts F,  
                   {act. Restrict (project_set h C) act 
-                          : project_act h ` Restrict C ` 
+                          \<in> project_act h ` Restrict C ` 
                                      (project_act h -` AllowedActs F)})"
 apply (rule program_equalityI)
   apply simp
@@ -439,7 +439,7 @@ apply (simp add: image_Un, auto)
 done
 
 lemma (in Extend) extend_JN [simp]:
-     "extend h (JOIN I F) = (JN i:I. extend h (F i))"
+     "extend h (JOIN I F) = (\<Squnion>i \<in> I. extend h (F i))"
 apply (rule program_equalityI)
   apply (simp (no_asm) add: extend_set_INT_distrib)
  apply (simp add: image_UN, auto)
@@ -447,49 +447,49 @@ done
 
 (** These monotonicity results look natural but are UNUSED **)
 
-lemma (in Extend) extend_mono: "F <= G ==> extend h F <= extend h G"
+lemma (in Extend) extend_mono: "F \<le> G ==> extend h F \<le> extend h G"
 by (force simp add: component_eq_subset)
 
-lemma (in Extend) project_mono: "F <= G ==> project h C F <= project h C G"
+lemma (in Extend) project_mono: "F \<le> G ==> project h C F \<le> project h C G"
 by (simp add: component_eq_subset, blast)
 
 
 subsection{*Safety: co, stable*}
 
 lemma (in Extend) extend_constrains:
-     "(extend h F : (extend_set h A) co (extend_set h B)) =  
-      (F : A co B)"
+     "(extend h F \<in> (extend_set h A) co (extend_set h B)) =  
+      (F \<in> A co B)"
 by (simp add: constrains_def)
 
 lemma (in Extend) extend_stable:
-     "(extend h F : stable (extend_set h A)) = (F : stable A)"
+     "(extend h F \<in> stable (extend_set h A)) = (F \<in> stable A)"
 by (simp add: stable_def extend_constrains)
 
 lemma (in Extend) extend_invariant:
-     "(extend h F : invariant (extend_set h A)) = (F : invariant A)"
+     "(extend h F \<in> invariant (extend_set h A)) = (F \<in> invariant A)"
 by (simp add: invariant_def extend_stable)
 
 (*Projects the state predicates in the property satisfied by  extend h F.
   Converse fails: A and B may differ in their extra variables*)
 lemma (in Extend) extend_constrains_project_set:
-     "extend h F : A co B ==> F : (project_set h A) co (project_set h B)"
+     "extend h F \<in> A co B ==> F \<in> (project_set h A) co (project_set h B)"
 by (auto simp add: constrains_def, force)
 
 lemma (in Extend) extend_stable_project_set:
-     "extend h F : stable A ==> F : stable (project_set h A)"
+     "extend h F \<in> stable A ==> F \<in> stable (project_set h A)"
 by (simp add: stable_def extend_constrains_project_set)
 
 
 subsection{*Weak safety primitives: Co, Stable*}
 
 lemma (in Extend) reachable_extend_f:
-     "p : reachable (extend h F) ==> f p : reachable F"
+     "p \<in> reachable (extend h F) ==> f p \<in> reachable F"
 apply (erule reachable.induct)
 apply (auto intro: reachable.intros simp add: extend_act_def image_iff)
 done
 
 lemma (in Extend) h_reachable_extend:
-     "h(s,y) : reachable (extend h F) ==> s : reachable F"
+     "h(s,y) \<in> reachable (extend h F) ==> s \<in> reachable F"
 by (force dest!: reachable_extend_f)
 
 lemma (in Extend) reachable_extend_eq: 
@@ -502,17 +502,17 @@ apply (force intro: reachable.intros)+
 done
 
 lemma (in Extend) extend_Constrains:
-     "(extend h F : (extend_set h A) Co (extend_set h B)) =   
-      (F : A Co B)"
+     "(extend h F \<in> (extend_set h A) Co (extend_set h B)) =   
+      (F \<in> A Co B)"
 by (simp add: Constrains_def reachable_extend_eq extend_constrains 
               extend_set_Int_distrib [symmetric])
 
 lemma (in Extend) extend_Stable:
-     "(extend h F : Stable (extend_set h A)) = (F : Stable A)"
+     "(extend h F \<in> Stable (extend_set h A)) = (F \<in> Stable A)"
 by (simp add: Stable_def extend_Constrains)
 
 lemma (in Extend) extend_Always:
-     "(extend h F : Always (extend_set h A)) = (F : Always A)"
+     "(extend h F \<in> Always (extend_set h A)) = (F \<in> Always A)"
 by (simp (no_asm_simp) add: Always_def extend_Stable)
 
 
@@ -521,24 +521,24 @@ by (simp (no_asm_simp) add: Always_def extend_Stable)
 (** projection: monotonicity for safety **)
 
 lemma project_act_mono:
-     "D <= C ==>  
-      project_act h (Restrict D act) <= project_act h (Restrict C act)"
+     "D \<subseteq> C ==>  
+      project_act h (Restrict D act) \<subseteq> project_act h (Restrict C act)"
 by (auto simp add: project_act_def)
 
 lemma (in Extend) project_constrains_mono:
-     "[| D <= C; project h C F : A co B |] ==> project h D F : A co B"
+     "[| D \<subseteq> C; project h C F \<in> A co B |] ==> project h D F \<in> A co B"
 apply (auto simp add: constrains_def)
 apply (drule project_act_mono, blast)
 done
 
 lemma (in Extend) project_stable_mono:
-     "[| D <= C;  project h C F : stable A |] ==> project h D F : stable A"
+     "[| D \<subseteq> C;  project h C F \<in> stable A |] ==> project h D F \<in> stable A"
 by (simp add: stable_def project_constrains_mono)
 
 (*Key lemma used in several proofs about project and co*)
 lemma (in Extend) project_constrains: 
-     "(project h C F : A co B)  =   
-      (F : (C Int extend_set h A) co (extend_set h B) & A <= B)"
+     "(project h C F \<in> A co B)  =   
+      (F \<in> (C \<inter> extend_set h A) co (extend_set h B) & A \<subseteq> B)"
 apply (unfold constrains_def)
 apply (auto intro!: project_act_I simp add: ball_Un)
 apply (force intro!: project_act_I dest!: subsetD)
@@ -548,46 +548,46 @@ apply (force dest!: subsetD)
 done
 
 lemma (in Extend) project_stable: 
-     "(project h UNIV F : stable A) = (F : stable (extend_set h A))"
+     "(project h UNIV F \<in> stable A) = (F \<in> stable (extend_set h A))"
 apply (unfold stable_def)
 apply (simp (no_asm) add: project_constrains)
 done
 
 lemma (in Extend) project_stable_I:
-     "F : stable (extend_set h A) ==> project h C F : stable A"
+     "F \<in> stable (extend_set h A) ==> project h C F \<in> stable A"
 apply (drule project_stable [THEN iffD2])
 apply (blast intro: project_stable_mono)
 done
 
 lemma (in Extend) Int_extend_set_lemma:
-     "A Int extend_set h ((project_set h A) Int B) = A Int extend_set h B"
+     "A \<inter> extend_set h ((project_set h A) \<inter> B) = A \<inter> extend_set h B"
 by (auto simp add: split_extended_all)
 
 (*Strange (look at occurrences of C) but used in leadsETo proofs*)
 lemma project_constrains_project_set:
-     "G : C co B ==> project h C G : project_set h C co project_set h B"
+     "G \<in> C co B ==> project h C G \<in> project_set h C co project_set h B"
 by (simp add: constrains_def project_def project_act_def, blast)
 
 lemma project_stable_project_set:
-     "G : stable C ==> project h C G : stable (project_set h C)"
+     "G \<in> stable C ==> project h C G \<in> stable (project_set h C)"
 by (simp add: stable_def project_constrains_project_set)
 
 
 subsection{*Progress: transient, ensures*}
 
 lemma (in Extend) extend_transient:
-     "(extend h F : transient (extend_set h A)) = (F : transient A)"
+     "(extend h F \<in> transient (extend_set h A)) = (F \<in> transient A)"
 by (auto simp add: transient_def extend_set_subset_Compl_eq Domain_extend_act)
 
 lemma (in Extend) extend_ensures:
-     "(extend h F : (extend_set h A) ensures (extend_set h B)) =  
-      (F : A ensures B)"
+     "(extend h F \<in> (extend_set h A) ensures (extend_set h B)) =  
+      (F \<in> A ensures B)"
 by (simp add: ensures_def extend_constrains extend_transient 
         extend_set_Un_distrib [symmetric] extend_set_Diff_distrib [symmetric])
 
 lemma (in Extend) leadsTo_imp_extend_leadsTo:
-     "F : A leadsTo B  
-      ==> extend h F : (extend_set h A) leadsTo (extend_set h B)"
+     "F \<in> A leadsTo B  
+      ==> extend h F \<in> (extend_set h A) leadsTo (extend_set h B)"
 apply (erule leadsTo_induct)
   apply (simp add: leadsTo_Basis extend_ensures)
  apply (blast intro: leadsTo_Trans)
@@ -596,21 +596,21 @@ done
 
 subsection{*Proving the converse takes some doing!*}
 
-lemma (in Extend) slice_iff [iff]: "(x : slice C y) = (h(x,y) : C)"
+lemma (in Extend) slice_iff [iff]: "(x \<in> slice C y) = (h(x,y) \<in> C)"
 by (simp (no_asm) add: slice_def)
 
-lemma (in Extend) slice_Union: "slice (Union S) y = (UN x:S. slice x y)"
+lemma (in Extend) slice_Union: "slice (Union S) y = (\<Union>x \<in> S. slice x y)"
 by auto
 
 lemma (in Extend) slice_extend_set: "slice (extend_set h A) y = A"
 by auto
 
 lemma (in Extend) project_set_is_UN_slice:
-     "project_set h A = (UN y. slice A y)"
+     "project_set h A = (\<Union>y. slice A y)"
 by auto
 
 lemma (in Extend) extend_transient_slice:
-     "extend h F : transient A ==> F : transient (slice A y)"
+     "extend h F \<in> transient A ==> F \<in> transient (slice A y)"
 apply (unfold transient_def, auto)
 apply (rule bexI, auto)
 apply (force simp add: extend_act_def)
@@ -618,25 +618,25 @@ done
 
 (*Converse?*)
 lemma (in Extend) extend_constrains_slice:
-     "extend h F : A co B ==> F : (slice A y) co (slice B y)"
+     "extend h F \<in> A co B ==> F \<in> (slice A y) co (slice B y)"
 by (auto simp add: constrains_def)
 
 lemma (in Extend) extend_ensures_slice:
-     "extend h F : A ensures B ==> F : (slice A y) ensures (project_set h B)"
+     "extend h F \<in> A ensures B ==> F \<in> (slice A y) ensures (project_set h B)"
 apply (auto simp add: ensures_def extend_constrains extend_transient)
 apply (erule_tac [2] extend_transient_slice [THEN transient_strengthen])
 apply (erule extend_constrains_slice [THEN constrains_weaken], auto)
 done
 
 lemma (in Extend) leadsTo_slice_project_set:
-     "ALL y. F : (slice B y) leadsTo CU ==> F : (project_set h B) leadsTo CU"
+     "\<forall>y. F \<in> (slice B y) leadsTo CU ==> F \<in> (project_set h B) leadsTo CU"
 apply (simp (no_asm) add: project_set_is_UN_slice)
 apply (blast intro: leadsTo_UN)
 done
 
 lemma (in Extend) extend_leadsTo_slice [rule_format]:
-     "extend h F : AU leadsTo BU  
-      ==> ALL y. F : (slice AU y) leadsTo (project_set h BU)"
+     "extend h F \<in> AU leadsTo BU  
+      ==> \<forall>y. F \<in> (slice AU y) leadsTo (project_set h BU)"
 apply (erule leadsTo_induct)
   apply (blast intro: extend_ensures_slice leadsTo_Basis)
  apply (blast intro: leadsTo_slice_project_set leadsTo_Trans)
@@ -644,8 +644,8 @@ apply (simp add: leadsTo_UN slice_Union)
 done
 
 lemma (in Extend) extend_leadsTo:
-     "(extend h F : (extend_set h A) leadsTo (extend_set h B)) =  
-      (F : A leadsTo B)"
+     "(extend h F \<in> (extend_set h A) leadsTo (extend_set h B)) =  
+      (F \<in> A leadsTo B)"
 apply safe
 apply (erule_tac [2] leadsTo_imp_extend_leadsTo)
 apply (drule extend_leadsTo_slice)
@@ -653,8 +653,8 @@ apply (simp add: slice_extend_set)
 done
 
 lemma (in Extend) extend_LeadsTo:
-     "(extend h F : (extend_set h A) LeadsTo (extend_set h B)) =   
-      (F : A LeadsTo B)"
+     "(extend h F \<in> (extend_set h A) LeadsTo (extend_set h B)) =   
+      (F \<in> A LeadsTo B)"
 by (simp add: LeadsTo_def reachable_extend_eq extend_leadsTo
               extend_set_Int_distrib [symmetric])
 
@@ -662,20 +662,20 @@ by (simp add: LeadsTo_def reachable_extend_eq extend_leadsTo
 subsection{*preserves*}
 
 lemma (in Extend) project_preserves_I:
-     "G : preserves (v o f) ==> project h C G : preserves v"
+     "G \<in> preserves (v o f) ==> project h C G \<in> preserves v"
 by (auto simp add: preserves_def project_stable_I extend_set_eq_Collect)
 
 (*to preserve f is to preserve the whole original state*)
 lemma (in Extend) project_preserves_id_I:
-     "G : preserves f ==> project h C G : preserves id"
+     "G \<in> preserves f ==> project h C G \<in> preserves id"
 by (simp add: project_preserves_I)
 
 lemma (in Extend) extend_preserves:
-     "(extend h G : preserves (v o f)) = (G : preserves v)"
+     "(extend h G \<in> preserves (v o f)) = (G \<in> preserves v)"
 by (auto simp add: preserves_def extend_stable [symmetric] 
                    extend_set_eq_Collect)
 
-lemma (in Extend) inj_extend_preserves: "inj h ==> (extend h G : preserves g)"
+lemma (in Extend) inj_extend_preserves: "inj h ==> (extend h G \<in> preserves g)"
 by (auto simp add: preserves_def extend_def extend_act_def stable_def 
                    constrains_def g_def)
 
@@ -719,16 +719,16 @@ apply (force+)
 done
 
 lemma (in Extend) guarantees_imp_extend_guarantees:
-     "F : X guarantees Y ==>  
-      extend h F : (extend h ` X) guarantees (extend h ` Y)"
+     "F \<in> X guarantees Y ==>  
+      extend h F \<in> (extend h ` X) guarantees (extend h ` Y)"
 apply (rule guaranteesI, clarify)
 apply (blast dest: ok_extend_imp_ok_project extend_Join_eq_extend_D 
                    guaranteesD)
 done
 
 lemma (in Extend) extend_guarantees_imp_guarantees:
-     "extend h F : (extend h ` X) guarantees (extend h ` Y)  
-      ==> F : X guarantees Y"
+     "extend h F \<in> (extend h ` X) guarantees (extend h ` Y)  
+      ==> F \<in> X guarantees Y"
 apply (auto simp add: guar_def)
 apply (drule_tac x = "extend h G" in spec)
 apply (simp del: extend_Join 
@@ -737,8 +737,8 @@ apply (simp del: extend_Join
 done
 
 lemma (in Extend) extend_guarantees_eq:
-     "(extend h F : (extend h ` X) guarantees (extend h ` Y)) =  
-      (F : X guarantees Y)"
+     "(extend h F \<in> (extend h ` X) guarantees (extend h ` Y)) =  
+      (F \<in> X guarantees Y)"
 by (blast intro: guarantees_imp_extend_guarantees 
                  extend_guarantees_imp_guarantees)
 
