src/HOL/UNITY/Follows.thy
@@ -12,22 +12,22 @@ constdefs
 
   Follows :: "['a => 'b::{order}, 'a => 'b::{order}] => 'a program set"
                  (infixl "Fols" 65)
-   "f Fols g == Increasing g Int Increasing f Int
-                Always {s. f s <= g s} Int
-                (INT k. {s. k <= g s} LeadsTo {s. k <= f s})"
+   "f Fols g == Increasing g \<inter> Increasing f Int
+                Always {s. f s \<le> g s} Int
+                (\<Inter>k. {s. k \<le> g s} LeadsTo {s. k \<le> f s})"
 
 
 (*Does this hold for "invariant"?*)
 lemma mono_Always_o:
-     "mono h ==> Always {s. f s <= g s} <= Always {s. h (f s) <= h (g s)}"
+     "mono h ==> Always {s. f s \<le> g s} \<subseteq> Always {s. h (f s) \<le> h (g s)}"
 apply (simp add: Always_eq_includes_reachable)
 apply (blast intro: monoD)
 done
 
 lemma mono_LeadsTo_o:
      "mono (h::'a::order => 'b::order)  
-      ==> (INT j. {s. j <= g s} LeadsTo {s. j <= f s}) <=  
-          (INT k. {s. k <= h (g s)} LeadsTo {s. k <= h (f s)})"
+      ==> (\<Inter>j. {s. j \<le> g s} LeadsTo {s. j \<le> f s}) \<subseteq>  
+          (\<Inter>k. {s. k \<le> h (g s)} LeadsTo {s. k \<le> h (f s)})"
 apply auto
 apply (rule single_LeadsTo_I)
 apply (drule_tac x = "g s" in spec)
@@ -35,10 +35,10 @@ apply (erule LeadsTo_weaken)
 apply (blast intro: monoD order_trans)+
 done
 
-lemma Follows_constant [iff]: "F : (%s. c) Fols (%s. c)"
+lemma Follows_constant [iff]: "F \<in> (%s. c) Fols (%s. c)"
 by (unfold Follows_def, auto)
 
-lemma mono_Follows_o: "mono h ==> f Fols g <= (h o f) Fols (h o g)"
+lemma mono_Follows_o: "mono h ==> f Fols g \<subseteq> (h o f) Fols (h o g)"
 apply (unfold Follows_def, clarify)
 apply (simp add: mono_Increasing_o [THEN [2] rev_subsetD]
                  mono_Always_o [THEN [2] rev_subsetD]
@@ -46,13 +46,13 @@ apply (simp add: mono_Increasing_o [THEN [2] rev_subsetD]
 done
 
 lemma mono_Follows_apply:
-     "mono h ==> f Fols g <= (%x. h (f x)) Fols (%x. h (g x))"
+     "mono h ==> f Fols g \<subseteq> (%x. h (f x)) Fols (%x. h (g x))"
 apply (drule mono_Follows_o)
 apply (force simp add: o_def)
 done
 
 lemma Follows_trans: 
-     "[| F : f Fols g;  F: g Fols h |] ==> F : f Fols h"
+     "[| F \<in> f Fols g;  F \<in> g Fols h |] ==> F \<in> f Fols h"
 apply (unfold Follows_def)
 apply (simp add: Always_eq_includes_reachable)
 apply (blast intro: order_trans LeadsTo_Trans)
@@ -61,24 +61,24 @@ done
 
 subsection{*Destruction rules*}
 
-lemma Follows_Increasing1: "F : f Fols g ==> F : Increasing f"
+lemma Follows_Increasing1: "F \<in> f Fols g ==> F \<in> Increasing f"
 apply (unfold Follows_def, blast)
 done
 
-lemma Follows_Increasing2: "F : f Fols g ==> F : Increasing g"
+lemma Follows_Increasing2: "F \<in> f Fols g ==> F \<in> Increasing g"
 apply (unfold Follows_def, blast)
 done
 
-lemma Follows_Bounded: "F : f Fols g ==> F : Always {s. f s <= g s}"
+lemma Follows_Bounded: "F \<in> f Fols g ==> F \<in> Always {s. f s \<subseteq> g s}"
 apply (unfold Follows_def, blast)
 done
 
 lemma Follows_LeadsTo: 
-     "F : f Fols g ==> F : {s. k <= g s} LeadsTo {s. k <= f s}"
+     "F \<in> f Fols g ==> F \<in> {s. k \<le> g s} LeadsTo {s. k \<le> f s}"
 by (unfold Follows_def, blast)
 
 lemma Follows_LeadsTo_pfixLe:
-     "F : f Fols g ==> F : {s. k pfixLe g s} LeadsTo {s. k pfixLe f s}"
+     "F \<in> f Fols g ==> F \<in> {s. k pfixLe g s} LeadsTo {s. k pfixLe f s}"
 apply (rule single_LeadsTo_I, clarify)
 apply (drule_tac k="g s" in Follows_LeadsTo)
 apply (erule LeadsTo_weaken)
@@ -87,7 +87,7 @@ apply (blast intro: pfixLe_trans prefix_imp_pfixLe)
 done
 
 lemma Follows_LeadsTo_pfixGe:
-     "F : f Fols g ==> F : {s. k pfixGe g s} LeadsTo {s. k pfixGe f s}"
+     "F \<in> f Fols g ==> F \<in> {s. k pfixGe g s} LeadsTo {s. k pfixGe f s}"
 apply (rule single_LeadsTo_I, clarify)
 apply (drule_tac k="g s" in Follows_LeadsTo)
 apply (erule LeadsTo_weaken)
@@ -97,21 +97,21 @@ done
 
 
 lemma Always_Follows1: 
-     "[| F : Always {s. f s = f' s}; F : f Fols g |] ==> F : f' Fols g"
+     "[| F \<in> Always {s. f s = f' s}; F \<in> f Fols g |] ==> F \<in> f' Fols g"
 
 apply (unfold Follows_def Increasing_def Stable_def, auto)
 apply (erule_tac [3] Always_LeadsTo_weaken)
-apply (erule_tac A = "{s. z <= f s}" and A' = "{s. z <= f s}" 
+apply (erule_tac A = "{s. z \<le> f s}" and A' = "{s. z \<le> f s}" 
        in Always_Constrains_weaken, auto)
 apply (drule Always_Int_I, assumption)
 apply (force intro: Always_weaken)
 done
 
 lemma Always_Follows2: 
-     "[| F : Always {s. g s = g' s}; F : f Fols g |] ==> F : f Fols g'"
+     "[| F \<in> Always {s. g s = g' s}; F \<in> f Fols g |] ==> F \<in> f Fols g'"
 apply (unfold Follows_def Increasing_def Stable_def, auto)
 apply (erule_tac [3] Always_LeadsTo_weaken)
-apply (erule_tac A = "{s. z <= g s}" and A' = "{s. z <= g s}"
+apply (erule_tac A = "{s. z \<le> g s}" and A' = "{s. z \<le> g s}"
        in Always_Constrains_weaken, auto)
 apply (drule Always_Int_I, assumption)
 apply (force intro: Always_weaken)
@@ -122,8 +122,8 @@ subsection{*Union properties (with the subset ordering)*}
 
 (*Can replace "Un" by any sup.  But existing max only works for linorders.*)
 lemma increasing_Un: 
-    "[| F : increasing f;  F: increasing g |]  
-     ==> F : increasing (%s. (f s) Un (g s))"
+    "[| F \<in> increasing f;  F \<in> increasing g |]  
+     ==> F \<in> increasing (%s. (f s) \<union> (g s))"
 apply (unfold increasing_def stable_def constrains_def, auto)
 apply (drule_tac x = "f xa" in spec)
 apply (drule_tac x = "g xa" in spec)
@@ -131,8 +131,8 @@ apply (blast dest!: bspec)
 done
 
 lemma Increasing_Un: 
-    "[| F : Increasing f;  F: Increasing g |]  
-     ==> F : Increasing (%s. (f s) Un (g s))"
+    "[| F \<in> Increasing f;  F \<in> Increasing g |]  
+     ==> F \<in> Increasing (%s. (f s) \<union> (g s))"
 apply (auto simp add: Increasing_def Stable_def Constrains_def
                       stable_def constrains_def)
 apply (drule_tac x = "f xa" in spec)
@@ -142,17 +142,17 @@ done
 
 
 lemma Always_Un:
-     "[| F : Always {s. f' s <= f s}; F : Always {s. g' s <= g s} |]  
-      ==> F : Always {s. f' s Un g' s <= f s Un g s}"
+     "[| F \<in> Always {s. f' s \<le> f s}; F \<in> Always {s. g' s \<le> g s} |]  
+      ==> F \<in> Always {s. f' s \<union> g' s \<le> f s \<union> g s}"
 by (simp add: Always_eq_includes_reachable, blast)
 
 (*Lemma to re-use the argument that one variable increases (progress)
   while the other variable doesn't decrease (safety)*)
 lemma Follows_Un_lemma:
-     "[| F : Increasing f; F : Increasing g;  
-         F : Increasing g'; F : Always {s. f' s <= f s}; 
-         ALL k. F : {s. k <= f s} LeadsTo {s. k <= f' s} |] 
-      ==> F : {s. k <= f s Un g s} LeadsTo {s. k <= f' s Un g s}"
+     "[| F \<in> Increasing f; F \<in> Increasing g;  
+         F \<in> Increasing g'; F \<in> Always {s. f' s \<le> f s}; 
+         \<forall>k. F \<in> {s. k \<le> f s} LeadsTo {s. k \<le> f' s} |] 
+      ==> F \<in> {s. k \<le> f s \<union> g s} LeadsTo {s. k \<le> f' s \<union> g s}"
 apply (rule single_LeadsTo_I)
 apply (drule_tac x = "f s" in IncreasingD)
 apply (drule_tac x = "g s" in IncreasingD)
@@ -164,8 +164,8 @@ apply blast+
 done
 
 lemma Follows_Un: 
-    "[| F : f' Fols f;  F: g' Fols g |]  
-     ==> F : (%s. (f' s) Un (g' s)) Fols (%s. (f s) Un (g s))"
+    "[| F \<in> f' Fols f;  F \<in> g' Fols g |]  
+     ==> F \<in> (%s. (f' s) \<union> (g' s)) Fols (%s. (f s) \<union> (g s))"
 apply (unfold Follows_def)
 apply (simp add: Increasing_Un Always_Un, auto)
 apply (rule LeadsTo_Trans)
@@ -178,8 +178,8 @@ done
 subsection{*Multiset union properties (with the multiset ordering)*}
 
 lemma increasing_union: 
-    "[| F : increasing f;  F: increasing g |]  
-     ==> F : increasing (%s. (f s) + (g s :: ('a::order) multiset))"
+    "[| F \<in> increasing f;  F \<in> increasing g |]  
+     ==> F \<in> increasing (%s. (f s) + (g s :: ('a::order) multiset))"
 apply (unfold increasing_def stable_def constrains_def, auto)
 apply (drule_tac x = "f xa" in spec)
 apply (drule_tac x = "g xa" in spec)
@@ -188,8 +188,8 @@ apply (blast intro: union_le_mono order_trans)
 done
 
 lemma Increasing_union: 
-    "[| F : Increasing f;  F: Increasing g |]  
-     ==> F : Increasing (%s. (f s) + (g s :: ('a::order) multiset))"
+    "[| F \<in> Increasing f;  F \<in> Increasing g |]  
+     ==> F \<in> Increasing (%s. (f s) + (g s :: ('a::order) multiset))"
 apply (auto simp add: Increasing_def Stable_def Constrains_def
                       stable_def constrains_def)
 apply (drule_tac x = "f xa" in spec)
@@ -199,19 +199,19 @@ apply (blast intro: union_le_mono order_trans)
 done
 
 lemma Always_union:
-     "[| F : Always {s. f' s <= f s}; F : Always {s. g' s <= g s} |]  
-      ==> F : Always {s. f' s + g' s <= f s + (g s :: ('a::order) multiset)}"
+     "[| F \<in> Always {s. f' s \<le> f s}; F \<in> Always {s. g' s \<le> g s} |]  
+      ==> F \<in> Always {s. f' s + g' s \<le> f s + (g s :: ('a::order) multiset)}"
 apply (simp add: Always_eq_includes_reachable)
 apply (blast intro: union_le_mono)
 done
 
 (*Except the last line, IDENTICAL to the proof script for Follows_Un_lemma*)
 lemma Follows_union_lemma:
-     "[| F : Increasing f; F : Increasing g;  
-         F : Increasing g'; F : Always {s. f' s <= f s}; 
-         ALL k::('a::order) multiset.  
-           F : {s. k <= f s} LeadsTo {s. k <= f' s} |] 
-      ==> F : {s. k <= f s + g s} LeadsTo {s. k <= f' s + g s}"
+     "[| F \<in> Increasing f; F \<in> Increasing g;  
+         F \<in> Increasing g'; F \<in> Always {s. f' s \<le> f s}; 
+         \<forall>k::('a::order) multiset.  
+           F \<in> {s. k \<le> f s} LeadsTo {s. k \<le> f' s} |] 
+      ==> F \<in> {s. k \<le> f s + g s} LeadsTo {s. k \<le> f' s + g s}"
 apply (rule single_LeadsTo_I)
 apply (drule_tac x = "f s" in IncreasingD)
 apply (drule_tac x = "g s" in IncreasingD)
@@ -226,8 +226,8 @@ done
 (*The !! is there to influence to effect of permutative rewriting at the end*)
 lemma Follows_union: 
      "!!g g' ::'b => ('a::order) multiset.  
-        [| F : f' Fols f;  F: g' Fols g |]  
-        ==> F : (%s. (f' s) + (g' s)) Fols (%s. (f s) + (g s))"
+        [| F \<in> f' Fols f;  F \<in> g' Fols g |]  
+        ==> F \<in> (%s. (f' s) + (g' s)) Fols (%s. (f s) + (g s))"
 apply (unfold Follows_def)
 apply (simp add: Increasing_union Always_union, auto)
 apply (rule LeadsTo_Trans)
@@ -239,8 +239,8 @@ done
 
 lemma Follows_setsum:
      "!!f ::['c,'b] => ('a::order) multiset.  
-        [| ALL i: I. F : f' i Fols f i;  finite I |]  
-        ==> F : (%s. \<Sum>i:I. f' i s) Fols (%s. \<Sum>i:I. f i s)"
+        [| \<forall>i \<in> I. F \<in> f' i Fols f i;  finite I |]  
+        ==> F \<in> (%s. \<Sum>i \<in> I. f' i s) Fols (%s. \<Sum>i \<in> I. f i s)"
 apply (erule rev_mp)
 apply (erule finite_induct, simp) 
 apply (simp add: Follows_union)
@@ -249,7 +249,7 @@ done
 
 (*Currently UNUSED, but possibly of interest*)
 lemma Increasing_imp_Stable_pfixGe:
-     "F : Increasing func ==> F : Stable {s. h pfixGe (func s)}"
+     "F \<in> Increasing func ==> F \<in> Stable {s. h pfixGe (func s)}"
 apply (simp add: Increasing_def Stable_def Constrains_def constrains_def)
 apply (blast intro: trans_Ge [THEN trans_genPrefix, THEN transD] 
                     prefix_imp_pfixGe)
@@ -257,8 +257,8 @@ done
 
 (*Currently UNUSED, but possibly of interest*)
 lemma LeadsTo_le_imp_pfixGe:
-     "ALL z. F : {s. z <= f s} LeadsTo {s. z <= g s}  
-      ==> F : {s. z pfixGe f s} LeadsTo {s. z pfixGe g s}"
+     "\<forall>z. F \<in> {s. z \<le> f s} LeadsTo {s. z \<le> g s}  
+      ==> F \<in> {s. z pfixGe f s} LeadsTo {s. z pfixGe g s}"
 apply (rule single_LeadsTo_I)
 apply (drule_tac x = "f s" in spec)
 apply (erule LeadsTo_weaken)
