src/HOL/UNITY/Guar.thy
@@ -32,57 +32,57 @@ constdefs
     case, proving equivalence with Chandy and Sanders's n-ary definitions*)
 
   ex_prop  :: "'a program set => bool"
-   "ex_prop X == \<forall>F G. F ok G -->F:X | G: X --> (F Join G) : X"
+   "ex_prop X == \<forall>F G. F ok G -->F \<in> X | G \<in> X --> (F Join G) \<in> X"
 
   strict_ex_prop  :: "'a program set => bool"
-   "strict_ex_prop X == \<forall>F G.  F ok G --> (F:X | G: X) = (F Join G : X)"
+   "strict_ex_prop X == \<forall>F G.  F ok G --> (F \<in> X | G \<in> X) = (F Join G \<in> X)"
 
   uv_prop  :: "'a program set => bool"
-   "uv_prop X == SKIP : X & (\<forall>F G. F ok G --> F:X & G: X --> (F Join G) : X)"
+   "uv_prop X == SKIP \<in> X & (\<forall>F G. F ok G --> F \<in> X & G \<in> X --> (F Join G) \<in> X)"
 
   strict_uv_prop  :: "'a program set => bool"
    "strict_uv_prop X == 
-      SKIP : X & (\<forall>F G. F ok G --> (F:X & G: X) = (F Join G : X))"
+      SKIP \<in> X & (\<forall>F G. F ok G --> (F \<in> X & G \<in> X) = (F Join G \<in> X))"
 
   guar :: "['a program set, 'a program set] => 'a program set"
           (infixl "guarantees" 55)  (*higher than membership, lower than Co*)
-   "X guarantees Y == {F. \<forall>G. F ok G --> F Join G : X --> F Join G : Y}"
+   "X guarantees Y == {F. \<forall>G. F ok G --> F Join G \<in> X --> F Join G \<in> Y}"
   
 
   (* Weakest guarantees *)
    wg :: "['a program, 'a program set] =>  'a program set"
-  "wg F Y == Union({X. F:X guarantees Y})"
+  "wg F Y == Union({X. F \<in> X guarantees Y})"
 
    (* Weakest existential property stronger than X *)
    wx :: "('a program) set => ('a program)set"
-   "wx X == Union({Y. Y<=X & ex_prop Y})"
+   "wx X == Union({Y. Y \<subseteq> X & ex_prop Y})"
   
   (*Ill-defined programs can arise through "Join"*)
   welldef :: "'a program set"
-  "welldef == {F. Init F ~= {}}"
+  "welldef == {F. Init F \<noteq> {}}"
   
   refines :: "['a program, 'a program, 'a program set] => bool"
 			("(3_ refines _ wrt _)" [10,10,10] 10)
   "G refines F wrt X ==
-     \<forall>H. (F ok H  & G ok H & F Join H : welldef Int X) --> 
-         (G Join H : welldef Int X)"
+     \<forall>H. (F ok H  & G ok H & F Join H \<in> welldef \<inter> X) --> 
+         (G Join H \<in> welldef \<inter> X)"
 
   iso_refines :: "['a program, 'a program, 'a program set] => bool"
                               ("(3_ iso'_refines _ wrt _)" [10,10,10] 10)
   "G iso_refines F wrt X ==
-   F : welldef Int X --> G : welldef Int X"
+   F \<in> welldef \<inter> X --> G \<in> welldef \<inter> X"
 
 
 lemma OK_insert_iff:
      "(OK (insert i I) F) = 
-      (if i:I then OK I F else OK I F & (F i ok JOIN I F))"
+      (if i \<in> I then OK I F else OK I F & (F i ok JOIN I F))"
 by (auto intro: ok_sym simp add: OK_iff_ok)
 
 
 (*** existential properties ***)
 lemma ex1 [rule_format]: 
  "[| ex_prop X; finite GG |] ==>  
-     GG Int X ~= {}--> OK GG (%G. G) -->(JN G:GG. G) : X"
+     GG \<inter> X \<noteq> {}--> OK GG (%G. G) --> (\<Squnion>G \<in> GG. G) \<in> X"
 apply (unfold ex_prop_def)
 apply (erule finite_induct)
 apply (auto simp add: OK_insert_iff Int_insert_left)
@@ -90,7 +90,7 @@ done
 
 
 lemma ex2: 
-     "\<forall>GG. finite GG & GG Int X ~= {} --> OK GG (%G. G) -->(JN G:GG. G):X 
+     "\<forall>GG. finite GG & GG \<inter> X \<noteq> {} --> OK GG (%G. G) -->(\<Squnion>G \<in> GG. G):X 
       ==> ex_prop X"
 apply (unfold ex_prop_def, clarify)
 apply (drule_tac x = "{F,G}" in spec)
@@ -101,13 +101,13 @@ done
 (*Chandy & Sanders take this as a definition*)
 lemma ex_prop_finite:
      "ex_prop X = 
-      (\<forall>GG. finite GG & GG Int X ~= {} & OK GG (%G. G)--> (JN G:GG. G) : X)"
+      (\<forall>GG. finite GG & GG \<inter> X \<noteq> {} & OK GG (%G. G)--> (\<Squnion>G \<in> GG. G) \<in> X)"
 by (blast intro: ex1 ex2)
 
 
 (*Their "equivalent definition" given at the end of section 3*)
 lemma ex_prop_equiv: 
-     "ex_prop X = (\<forall>G. G:X = (\<forall>H. (G component_of H) --> H: X))"
+     "ex_prop X = (\<forall>G. G \<in> X = (\<forall>H. (G component_of H) --> H \<in> X))"
 apply auto
 apply (unfold ex_prop_def component_of_def, safe)
 apply blast 
@@ -120,14 +120,14 @@ done
 (*** universal properties ***)
 lemma uv1 [rule_format]: 
      "[| uv_prop X; finite GG |] 
-      ==> GG <= X & OK GG (%G. G) --> (JN G:GG. G) : X"
+      ==> GG \<subseteq> X & OK GG (%G. G) --> (\<Squnion>G \<in> GG. G) \<in> X"
 apply (unfold uv_prop_def)
 apply (erule finite_induct)
 apply (auto simp add: Int_insert_left OK_insert_iff)
 done
 
 lemma uv2: 
-     "\<forall>GG. finite GG & GG <= X & OK GG (%G. G) --> (JN G:GG. G) : X  
+     "\<forall>GG. finite GG & GG \<subseteq> X & OK GG (%G. G) --> (\<Squnion>G \<in> GG. G) \<in> X  
       ==> uv_prop X"
 apply (unfold uv_prop_def)
 apply (rule conjI)
@@ -141,37 +141,37 @@ done
 (*Chandy & Sanders take this as a definition*)
 lemma uv_prop_finite:
      "uv_prop X = 
-      (\<forall>GG. finite GG & GG <= X & OK GG (%G. G) --> (JN G:GG. G): X)"
+      (\<forall>GG. finite GG & GG \<subseteq> X & OK GG (%G. G) --> (\<Squnion>G \<in> GG. G): X)"
 by (blast intro: uv1 uv2)
 
 (*** guarantees ***)
 
 lemma guaranteesI:
-     "(!!G. [| F ok G; F Join G : X |] ==> F Join G : Y)  
-      ==> F : X guarantees Y"
+     "(!!G. [| F ok G; F Join G \<in> X |] ==> F Join G \<in> Y)  
+      ==> F \<in> X guarantees Y"
 by (simp add: guar_def component_def)
 
 lemma guaranteesD: 
-     "[| F : X guarantees Y;  F ok G;  F Join G : X |]  
-      ==> F Join G : Y"
+     "[| F \<in> X guarantees Y;  F ok G;  F Join G \<in> X |]  
+      ==> F Join G \<in> Y"
 by (unfold guar_def component_def, blast)
 
 (*This version of guaranteesD matches more easily in the conclusion
-  The major premise can no longer be  F<=H since we need to reason about G*)
+  The major premise can no longer be  F \<subseteq> H since we need to reason about G*)
 lemma component_guaranteesD: 
-     "[| F : X guarantees Y;  F Join G = H;  H : X;  F ok G |]  
-      ==> H : Y"
+     "[| F \<in> X guarantees Y;  F Join G = H;  H \<in> X;  F ok G |]  
+      ==> H \<in> Y"
 by (unfold guar_def, blast)
 
 lemma guarantees_weaken: 
-     "[| F: X guarantees X'; Y <= X; X' <= Y' |] ==> F: Y guarantees Y'"
+     "[| F \<in> X guarantees X'; Y \<subseteq> X; X' \<subseteq> Y' |] ==> F \<in> Y guarantees Y'"
 by (unfold guar_def, blast)
 
-lemma subset_imp_guarantees_UNIV: "X <= Y ==> X guarantees Y = UNIV"
+lemma subset_imp_guarantees_UNIV: "X \<subseteq> Y ==> X guarantees Y = UNIV"
 by (unfold guar_def, blast)
 
 (*Equivalent to subset_imp_guarantees_UNIV but more intuitive*)
-lemma subset_imp_guarantees: "X <= Y ==> F : X guarantees Y"
+lemma subset_imp_guarantees: "X \<subseteq> Y ==> F \<in> X guarantees Y"
 by (unfold guar_def, blast)
 
 (*Remark at end of section 4.1 *)
@@ -201,31 +201,31 @@ done
 (** Distributive laws.  Re-orient to perform miniscoping **)
 
 lemma guarantees_UN_left: 
-     "(UN i:I. X i) guarantees Y = (INT i:I. X i guarantees Y)"
+     "(\<Union>i \<in> I. X i) guarantees Y = (\<Inter>i \<in> I. X i guarantees Y)"
 by (unfold guar_def, blast)
 
 lemma guarantees_Un_left: 
-     "(X Un Y) guarantees Z = (X guarantees Z) Int (Y guarantees Z)"
+     "(X \<union> Y) guarantees Z = (X guarantees Z) \<inter> (Y guarantees Z)"
 by (unfold guar_def, blast)
 
 lemma guarantees_INT_right: 
-     "X guarantees (INT i:I. Y i) = (INT i:I. X guarantees Y i)"
+     "X guarantees (\<Inter>i \<in> I. Y i) = (\<Inter>i \<in> I. X guarantees Y i)"
 by (unfold guar_def, blast)
 
 lemma guarantees_Int_right: 
-     "Z guarantees (X Int Y) = (Z guarantees X) Int (Z guarantees Y)"
+     "Z guarantees (X \<inter> Y) = (Z guarantees X) \<inter> (Z guarantees Y)"
 by (unfold guar_def, blast)
 
 lemma guarantees_Int_right_I:
-     "[| F : Z guarantees X;  F : Z guarantees Y |]  
-     ==> F : Z guarantees (X Int Y)"
+     "[| F \<in> Z guarantees X;  F \<in> Z guarantees Y |]  
+     ==> F \<in> Z guarantees (X \<inter> Y)"
 by (simp add: guarantees_Int_right)
 
 lemma guarantees_INT_right_iff:
-     "(F : X guarantees (INTER I Y)) = (\<forall>i\<in>I. F : X guarantees (Y i))"
+     "(F \<in> X guarantees (INTER I Y)) = (\<forall>i\<in>I. F \<in> X guarantees (Y i))"
 by (simp add: guarantees_INT_right)
 
-lemma shunting: "(X guarantees Y) = (UNIV guarantees (-X Un Y))"
+lemma shunting: "(X guarantees Y) = (UNIV guarantees (-X \<union> Y))"
 by (unfold guar_def, blast)
 
 lemma contrapositive: "(X guarantees Y) = -Y guarantees -X"
@@ -236,35 +236,35 @@ by (unfold guar_def, blast)
 **)
 
 lemma combining1: 
-    "[| F : V guarantees X;  F : (X Int Y) guarantees Z |] 
-     ==> F : (V Int Y) guarantees Z"
+    "[| F \<in> V guarantees X;  F \<in> (X \<inter> Y) guarantees Z |] 
+     ==> F \<in> (V \<inter> Y) guarantees Z"
 
 by (unfold guar_def, blast)
 
 lemma combining2: 
-    "[| F : V guarantees (X Un Y);  F : Y guarantees Z |] 
-     ==> F : V guarantees (X Un Z)"
+    "[| F \<in> V guarantees (X \<union> Y);  F \<in> Y guarantees Z |] 
+     ==> F \<in> V guarantees (X \<union> Z)"
 by (unfold guar_def, blast)
 
 (** The following two follow Chandy-Sanders, but the use of object-quantifiers
     does not suit Isabelle... **)
 
-(*Premise should be (!!i. i: I ==> F: X guarantees Y i) *)
+(*Premise should be (!!i. i \<in> I ==> F \<in> X guarantees Y i) *)
 lemma all_guarantees: 
-     "\<forall>i\<in>I. F : X guarantees (Y i) ==> F : X guarantees (INT i:I. Y i)"
+     "\<forall>i\<in>I. F \<in> X guarantees (Y i) ==> F \<in> X guarantees (\<Inter>i \<in> I. Y i)"
 by (unfold guar_def, blast)
 
-(*Premises should be [| F: X guarantees Y i; i: I |] *)
+(*Premises should be [| F \<in> X guarantees Y i; i \<in> I |] *)
 lemma ex_guarantees: 
-     "\<exists>i\<in>I. F : X guarantees (Y i) ==> F : X guarantees (UN i:I. Y i)"
+     "\<exists>i\<in>I. F \<in> X guarantees (Y i) ==> F \<in> X guarantees (\<Union>i \<in> I. Y i)"
 by (unfold guar_def, blast)
 
 
 (*** Additional guarantees laws, by lcp ***)
 
 lemma guarantees_Join_Int: 
-    "[| F: U guarantees V;  G: X guarantees Y; F ok G |]  
-     ==> F Join G: (U Int X) guarantees (V Int Y)"
+    "[| F \<in> U guarantees V;  G \<in> X guarantees Y; F ok G |]  
+     ==> F Join G \<in> (U \<inter> X) guarantees (V \<inter> Y)"
 apply (unfold guar_def)
 apply (simp (no_asm))
 apply safe
@@ -275,8 +275,8 @@ apply (simp (no_asm_simp) add: Join_ac)
 done
 
 lemma guarantees_Join_Un: 
-    "[| F: U guarantees V;  G: X guarantees Y; F ok G |]   
-     ==> F Join G: (U Un X) guarantees (V Un Y)"
+    "[| F \<in> U guarantees V;  G \<in> X guarantees Y; F ok G |]   
+     ==> F Join G \<in> (U \<union> X) guarantees (V \<union> Y)"
 apply (unfold guar_def)
 apply (simp (no_asm))
 apply safe
@@ -287,8 +287,8 @@ apply (simp (no_asm_simp) add: Join_ac)
 done
 
 lemma guarantees_JN_INT: 
-     "[| \<forall>i\<in>I. F i : X i guarantees Y i;  OK I F |]  
-      ==> (JOIN I F) : (INTER I X) guarantees (INTER I Y)"
+     "[| \<forall>i\<in>I. F i \<in> X i guarantees Y i;  OK I F |]  
+      ==> (JOIN I F) \<in> (INTER I X) guarantees (INTER I Y)"
 apply (unfold guar_def, auto)
 apply (drule bspec, assumption)
 apply (rename_tac "i")
@@ -298,8 +298,8 @@ apply (auto intro: OK_imp_ok
 done
 
 lemma guarantees_JN_UN: 
-    "[| \<forall>i\<in>I. F i : X i guarantees Y i;  OK I F |]  
-     ==> (JOIN I F) : (UNION I X) guarantees (UNION I Y)"
+    "[| \<forall>i\<in>I. F i \<in> X i guarantees Y i;  OK I F |]  
+     ==> (JOIN I F) \<in> (UNION I X) guarantees (UNION I Y)"
 apply (unfold guar_def, auto)
 apply (drule bspec, assumption)
 apply (rename_tac "i")
@@ -312,7 +312,7 @@ done
 (*** guarantees laws for breaking down the program, by lcp ***)
 
 lemma guarantees_Join_I1: 
-     "[| F: X guarantees Y;  F ok G |] ==> F Join G: X guarantees Y"
+     "[| F \<in> X guarantees Y;  F ok G |] ==> F Join G \<in> X guarantees Y"
 apply (unfold guar_def)
 apply (simp (no_asm))
 apply safe
@@ -320,14 +320,14 @@ apply (simp add: Join_assoc)
 done
 
 lemma guarantees_Join_I2:
-     "[| G: X guarantees Y;  F ok G |] ==> F Join G: X guarantees Y"
+     "[| G \<in> X guarantees Y;  F ok G |] ==> F Join G \<in> X guarantees Y"
 apply (simp add: Join_commute [of _ G] ok_commute [of _ G])
 apply (blast intro: guarantees_Join_I1)
 done
 
 lemma guarantees_JN_I: 
-     "[| i : I;  F i: X guarantees Y;  OK I F |]  
-      ==> (JN i:I. (F i)) : X guarantees Y"
+     "[| i \<in> I;  F i \<in> X guarantees Y;  OK I F |]  
+      ==> (\<Squnion>i \<in> I. (F i)) \<in> X guarantees Y"
 apply (unfold guar_def, clarify)
 apply (drule_tac x = "JOIN (I-{i}) F Join G" in spec)
 apply (auto intro: OK_imp_ok simp add: JN_Join_diff JN_Join_diff Join_assoc [symmetric])
@@ -336,10 +336,10 @@ done
 
 (*** well-definedness ***)
 
-lemma Join_welldef_D1: "F Join G: welldef ==> F: welldef"
+lemma Join_welldef_D1: "F Join G \<in> welldef ==> F \<in> welldef"
 by (unfold welldef_def, auto)
 
-lemma Join_welldef_D2: "F Join G: welldef ==> G: welldef"
+lemma Join_welldef_D2: "F Join G \<in> welldef ==> G \<in> welldef"
 by (unfold welldef_def, auto)
 
 (*** refinement ***)
@@ -357,14 +357,14 @@ qed "refines_trans"; *)
 
 lemma strict_ex_refine_lemma: 
      "strict_ex_prop X  
-      ==> (\<forall>H. F ok H & G ok H & F Join H : X --> G Join H : X)  
-              = (F:X --> G:X)"
+      ==> (\<forall>H. F ok H & G ok H & F Join H \<in> X --> G Join H \<in> X)  
+              = (F \<in> X --> G \<in> X)"
 by (unfold strict_ex_prop_def, auto)
 
 lemma strict_ex_refine_lemma_v: 
      "strict_ex_prop X  
-      ==> (\<forall>H. F ok H & G ok H & F Join H : welldef & F Join H : X --> G Join H : X) =  
-          (F: welldef Int X --> G:X)"
+      ==> (\<forall>H. F ok H & G ok H & F Join H \<in> welldef & F Join H \<in> X --> G Join H \<in> X) =  
+          (F \<in> welldef \<inter> X --> G \<in> X)"
 apply (unfold strict_ex_prop_def, safe)
 apply (erule_tac x = SKIP and P = "%H. ?PP H --> ?RR H" in allE)
 apply (auto dest: Join_welldef_D1 Join_welldef_D2)
@@ -372,7 +372,7 @@ done
 
 lemma ex_refinement_thm:
      "[| strict_ex_prop X;   
-         \<forall>H. F ok H & G ok H & F Join H : welldef Int X --> G Join H : welldef |]  
+         \<forall>H. F ok H & G ok H & F Join H \<in> welldef \<inter> X --> G Join H \<in> welldef |]  
       ==> (G refines F wrt X) = (G iso_refines F wrt X)"
 apply (rule_tac x = SKIP in allE, assumption)
 apply (simp add: refines_def iso_refines_def strict_ex_refine_lemma_v)
@@ -381,13 +381,13 @@ done
 
 lemma strict_uv_refine_lemma: 
      "strict_uv_prop X ==> 
-      (\<forall>H. F ok H & G ok H & F Join H : X --> G Join H : X) = (F:X --> G:X)"
+      (\<forall>H. F ok H & G ok H & F Join H \<in> X --> G Join H \<in> X) = (F \<in> X --> G \<in> X)"
 by (unfold strict_uv_prop_def, blast)
 
 lemma strict_uv_refine_lemma_v: 
      "strict_uv_prop X  
-      ==> (\<forall>H. F ok H & G ok H & F Join H : welldef & F Join H : X --> G Join H : X) =  
-          (F: welldef Int X --> G:X)"
+      ==> (\<forall>H. F ok H & G ok H & F Join H \<in> welldef & F Join H \<in> X --> G Join H \<in> X) =  
+          (F \<in> welldef \<inter> X --> G \<in> X)"
 apply (unfold strict_uv_prop_def, safe)
 apply (erule_tac x = SKIP and P = "%H. ?PP H --> ?RR H" in allE)
 apply (auto dest: Join_welldef_D1 Join_welldef_D2)
@@ -395,8 +395,8 @@ done
 
 lemma uv_refinement_thm:
      "[| strict_uv_prop X;   
-         \<forall>H. F ok H & G ok H & F Join H : welldef Int X --> 
-             G Join H : welldef |]  
+         \<forall>H. F ok H & G ok H & F Join H \<in> welldef \<inter> X --> 
+             G Join H \<in> welldef |]  
       ==> (G refines F wrt X) = (G iso_refines F wrt X)"
 apply (rule_tac x = SKIP in allE, assumption)
 apply (simp add: refines_def iso_refines_def strict_uv_refine_lemma_v)
@@ -404,17 +404,17 @@ done
 
 (* Added by Sidi Ehmety from Chandy & Sander, section 6 *)
 lemma guarantees_equiv: 
-    "(F:X guarantees Y) = (\<forall>H. H:X \<longrightarrow> (F component_of H \<longrightarrow> H:Y))"
+    "(F \<in> X guarantees Y) = (\<forall>H. H \<in> X \<longrightarrow> (F component_of H \<longrightarrow> H \<in> Y))"
 by (unfold guar_def component_of_def, auto)
 
-lemma wg_weakest: "!!X. F:(X guarantees Y) ==> X <= (wg F Y)"
+lemma wg_weakest: "!!X. F:(X guarantees Y) ==> X \<subseteq> (wg F Y)"
 by (unfold wg_def, auto)
 
 lemma wg_guarantees: "F:((wg F Y) guarantees Y)"
 by (unfold wg_def guar_def, blast)
 
 lemma wg_equiv: 
-  "(H: wg F X) = (F component_of H --> H:X)"
+  "(H \<in> wg F X) = (F component_of H --> H \<in> X)"
 apply (unfold wg_def)
 apply (simp (no_asm) add: guarantees_equiv)
 apply (rule iffI)
@@ -423,21 +423,21 @@ apply (blast+)
 done
 
 
-lemma component_of_wg: "F component_of H ==> (H:wg F X) = (H:X)"
+lemma component_of_wg: "F component_of H ==> (H \<in> wg F X) = (H \<in> X)"
 by (simp add: wg_equiv)
 
 lemma wg_finite: 
-    "\<forall>FF. finite FF & FF Int X ~= {} --> OK FF (%F. F)  
-          --> (\<forall>F\<in>FF. ((JN F:FF. F): wg F X) = ((JN F:FF. F):X))"
+    "\<forall>FF. finite FF & FF \<inter> X \<noteq> {} --> OK FF (%F. F)  
+          --> (\<forall>F\<in>FF. ((\<Squnion>F \<in> FF. F): wg F X) = ((\<Squnion>F \<in> FF. F):X))"
 apply clarify
-apply (subgoal_tac "F component_of (JN F:FF. F) ")
+apply (subgoal_tac "F component_of (\<Squnion>F \<in> FF. F) ")
 apply (drule_tac X = X in component_of_wg, simp)
 apply (simp add: component_of_def)
-apply (rule_tac x = "JN F: (FF-{F}) . F" in exI)
+apply (rule_tac x = "\<Squnion>F \<in> (FF-{F}) . F" in exI)
 apply (auto intro: JN_Join_diff dest: ok_sym simp add: OK_iff_ok)
 done
 
-lemma wg_ex_prop: "ex_prop X ==> (F:X) = (\<forall>H. H : wg F X)"
+lemma wg_ex_prop: "ex_prop X ==> (F \<in> X) = (\<forall>H. H \<in> wg F X)"
 apply (simp (no_asm_use) add: ex_prop_equiv wg_equiv)
 apply blast
 done
@@ -455,11 +455,11 @@ apply blast
 apply auto
 done
 
-lemma wx_weakest: "\<forall>Z. Z<= X --> ex_prop Z --> Z <= wx X"
+lemma wx_weakest: "\<forall>Z. Z<= X --> ex_prop Z --> Z \<subseteq> wx X"
 by (unfold wx_def, auto)
 
 (* Proposition 6 *)
-lemma wx'_ex_prop: "ex_prop({F. \<forall>G. F ok G --> F Join G:X})"
+lemma wx'_ex_prop: "ex_prop({F. \<forall>G. F ok G --> F Join G \<in> X})"
 apply (unfold ex_prop_def, safe)
 apply (drule_tac x = "G Join Ga" in spec)
 apply (force simp add: ok_Join_iff1 Join_assoc)
@@ -483,7 +483,7 @@ apply (drule_tac x = x in spec)
 apply (drule_tac x = G in spec)
 apply (frule_tac c = "x Join G" in subsetD, safe)
 apply (simp (no_asm))
-apply (rule_tac x = "{F. \<forall>G. F ok G --> F Join G:X}" in exI, safe)
+apply (rule_tac x = "{F. \<forall>G. F ok G --> F Join G \<in> X}" in exI, safe)
 apply (rule_tac [2] wx'_ex_prop)
 apply (rotate_tac 1)
 apply (drule_tac x = SKIP in spec, auto)
@@ -496,7 +496,7 @@ done
 (* Proposition 12 *)
 (* Main result of the paper *)
 lemma guarantees_wx_eq: 
-   "(X guarantees Y) = wx(-X Un Y)"
+   "(X guarantees Y) = wx(-X \<union> Y)"
 apply (unfold guar_def)
 apply (simp (no_asm) add: wx_equiv)
 done
@@ -511,7 +511,7 @@ done
     Reasoning About Program composition paper *)
 
 lemma stable_guarantees_Always:
-     "Init F <= A ==> F:(stable A) guarantees (Always A)"
+     "Init F \<subseteq> A ==> F:(stable A) guarantees (Always A)"
 apply (rule guaranteesI)
 apply (simp (no_asm) add: Join_commute)
 apply (rule stable_Join_Always1)
@@ -519,7 +519,7 @@ apply (simp_all add: invariant_def Join_stable)
 done
 
 (* To be moved to WFair.ML *)
-lemma leadsTo_Basis': "[| F:A co A Un B; F:transient A |] ==> F:A leadsTo B"
+lemma leadsTo_Basis': "[| F \<in> A co A \<union> B; F \<in> transient A |] ==> F \<in> A leadsTo B"
 apply (drule_tac B = "A-B" in constrains_weaken_L)
 apply (drule_tac [2] B = "A-B" in transient_strengthen)
 apply (rule_tac [3] ensuresI [THEN leadsTo_Basis])
@@ -529,7 +529,7 @@ done
 
 
 lemma constrains_guarantees_leadsTo:
-     "F : transient A ==> F: (A co A Un B) guarantees (A leadsTo (B-A))"
+     "F \<in> transient A ==> F \<in> (A co A \<union> B) guarantees (A leadsTo (B-A))"
 apply (rule guaranteesI)
 apply (rule leadsTo_Basis')
 apply (drule constrains_weaken_R)
