src/HOL/UNITY/Union.thy
@@ -12,36 +12,36 @@ theory Union = SubstAx + FP:
 
 constdefs
 
-  (*FIXME: conjoin Init F Int Init G ~= {} *) 
+  (*FIXME: conjoin Init F \<inter> Init G \<noteq> {} *) 
   ok :: "['a program, 'a program] => bool"      (infixl "ok" 65)
-    "F ok G == Acts F <= AllowedActs G &
-               Acts G <= AllowedActs F"
+    "F ok G == Acts F \<subseteq> AllowedActs G &
+               Acts G \<subseteq> AllowedActs F"
 
-  (*FIXME: conjoin (INT i:I. Init (F i)) ~= {} *) 
+  (*FIXME: conjoin (\<Inter>i \<in> I. Init (F i)) \<noteq> {} *) 
   OK  :: "['a set, 'a => 'b program] => bool"
-    "OK I F == (ALL i:I. ALL j: I-{i}. Acts (F i) <= AllowedActs (F j))"
+    "OK I F == (\<forall>i \<in> I. \<forall>j \<in> I-{i}. Acts (F i) \<subseteq> AllowedActs (F j))"
 
   JOIN  :: "['a set, 'a => 'b program] => 'b program"
-    "JOIN I F == mk_program (INT i:I. Init (F i), UN i:I. Acts (F i),
-			     INT i:I. AllowedActs (F i))"
+    "JOIN I F == mk_program (\<Inter>i \<in> I. Init (F i), \<Union>i \<in> I. Acts (F i),
+			     \<Inter>i \<in> I. AllowedActs (F i))"
 
   Join :: "['a program, 'a program] => 'a program"      (infixl "Join" 65)
-    "F Join G == mk_program (Init F Int Init G, Acts F Un Acts G,
-			     AllowedActs F Int AllowedActs G)"
+    "F Join G == mk_program (Init F \<inter> Init G, Acts F \<union> Acts G,
+			     AllowedActs F \<inter> AllowedActs G)"
 
   SKIP :: "'a program"
     "SKIP == mk_program (UNIV, {}, UNIV)"
 
   (*Characterizes safety properties.  Used with specifying AllowedActs*)
   safety_prop :: "'a program set => bool"
-    "safety_prop X == SKIP: X & (ALL G. Acts G <= UNION X Acts --> G : X)"
+    "safety_prop X == SKIP: X & (\<forall>G. Acts G \<subseteq> UNION X Acts --> G \<in> X)"
 
 syntax
   "@JOIN1"     :: "[pttrns, 'b set] => 'b set"         ("(3JN _./ _)" 10)
   "@JOIN"      :: "[pttrn, 'a set, 'b set] => 'b set"  ("(3JN _:_./ _)" 10)
 
 translations
-  "JN x:A. B"   == "JOIN A (%x. B)"
+  "JN x : A. B"   == "JOIN A (%x. B)"
   "JN x y. B"   == "JN x. JN y. B"
   "JN x. B"     == "JOIN UNIV (%x. B)"
 
@@ -49,7 +49,7 @@ syntax (xsymbols)
   SKIP      :: "'a program"                              ("\<bottom>")
   "op Join" :: "['a program, 'a program] => 'a program"  (infixl "\<squnion>" 65)
   "@JOIN1"  :: "[pttrns, 'b set] => 'b set"              ("(3\<Squnion> _./ _)" 10)
-  "@JOIN"   :: "[pttrn, 'a set, 'b set] => 'b set"       ("(3\<Squnion> _:_./ _)" 10)
+  "@JOIN"   :: "[pttrn, 'a set, 'b set] => 'b set"       ("(3\<Squnion> _\<in>_./ _)" 10)
 
 
 subsection{*SKIP*}
@@ -68,13 +68,13 @@ by (force elim: reachable.induct intro: reachable.intros)
 
 subsection{*SKIP and safety properties*}
 
-lemma SKIP_in_constrains_iff [iff]: "(SKIP : A co B) = (A<=B)"
+lemma SKIP_in_constrains_iff [iff]: "(SKIP \<in> A co B) = (A \<subseteq> B)"
 by (unfold constrains_def, auto)
 
-lemma SKIP_in_Constrains_iff [iff]: "(SKIP : A Co B) = (A<=B)"
+lemma SKIP_in_Constrains_iff [iff]: "(SKIP \<in> A Co B) = (A \<subseteq> B)"
 by (unfold Constrains_def, auto)
 
-lemma SKIP_in_stable [iff]: "SKIP : stable A"
+lemma SKIP_in_stable [iff]: "SKIP \<in> stable A"
 by (unfold stable_def, auto)
 
 declare SKIP_in_stable [THEN stable_imp_Stable, iff]
@@ -82,40 +82,40 @@ declare SKIP_in_stable [THEN stable_imp_Stable, iff]
 
 subsection{*Join*}
 
-lemma Init_Join [simp]: "Init (F Join G) = Init F Int Init G"
+lemma Init_Join [simp]: "Init (F Join G) = Init F \<inter> Init G"
 by (simp add: Join_def)
 
-lemma Acts_Join [simp]: "Acts (F Join G) = Acts F Un Acts G"
+lemma Acts_Join [simp]: "Acts (F Join G) = Acts F \<union> Acts G"
 by (auto simp add: Join_def)
 
 lemma AllowedActs_Join [simp]:
-     "AllowedActs (F Join G) = AllowedActs F Int AllowedActs G"
+     "AllowedActs (F Join G) = AllowedActs F \<inter> AllowedActs G"
 by (auto simp add: Join_def)
 
 
 subsection{*JN*}
 
-lemma JN_empty [simp]: "(JN i:{}. F i) = SKIP"
+lemma JN_empty [simp]: "(\<Squnion>i\<in>{}. F i) = SKIP"
 by (unfold JOIN_def SKIP_def, auto)
 
-lemma JN_insert [simp]: "(JN i:insert a I. F i) = (F a) Join (JN i:I. F i)"
+lemma JN_insert [simp]: "(\<Squnion>i \<in> insert a I. F i) = (F a) Join (\<Squnion>i \<in> I. F i)"
 apply (rule program_equalityI)
 apply (auto simp add: JOIN_def Join_def)
 done
 
-lemma Init_JN [simp]: "Init (JN i:I. F i) = (INT i:I. Init (F i))"
+lemma Init_JN [simp]: "Init (\<Squnion>i \<in> I. F i) = (\<Inter>i \<in> I. Init (F i))"
 by (simp add: JOIN_def)
 
-lemma Acts_JN [simp]: "Acts (JN i:I. F i) = insert Id (UN i:I. Acts (F i))"
+lemma Acts_JN [simp]: "Acts (\<Squnion>i \<in> I. F i) = insert Id (\<Union>i \<in> I. Acts (F i))"
 by (auto simp add: JOIN_def)
 
 lemma AllowedActs_JN [simp]:
-     "AllowedActs (JN i:I. F i) = (INT i:I. AllowedActs (F i))"
+     "AllowedActs (\<Squnion>i \<in> I. F i) = (\<Inter>i \<in> I. AllowedActs (F i))"
 by (auto simp add: JOIN_def)
 
 
 lemma JN_cong [cong]: 
-    "[| I=J;  !!i. i:J ==> F i = G i |] ==> (JN i:I. F i) = (JN i:J. G i)"
+    "[| I=J;  !!i. i \<in> J ==> F i = G i |] ==> (\<Squnion>i \<in> I. F i) = (\<Squnion>i \<in> J. G i)"
 by (simp add: JOIN_def)
 
 
@@ -156,28 +156,28 @@ done
 lemmas Join_ac = Join_assoc Join_left_absorb Join_commute Join_left_commute
 
 
-subsection{*JN laws*}
+subsection{*\<Squnion>laws*}
 
 (*Also follows by JN_insert and insert_absorb, but the proof is longer*)
-lemma JN_absorb: "k:I ==> F k Join (JN i:I. F i) = (JN i:I. F i)"
+lemma JN_absorb: "k \<in> I ==> F k Join (\<Squnion>i \<in> I. F i) = (\<Squnion>i \<in> I. F i)"
 by (auto intro!: program_equalityI)
 
-lemma JN_Un: "(JN i: I Un J. F i) = ((JN i: I. F i) Join (JN i:J. F i))"
+lemma JN_Un: "(\<Squnion>i \<in> I \<union> J. F i) = ((\<Squnion>i \<in> I. F i) Join (\<Squnion>i \<in> J. F i))"
 by (auto intro!: program_equalityI)
 
-lemma JN_constant: "(JN i:I. c) = (if I={} then SKIP else c)"
+lemma JN_constant: "(\<Squnion>i \<in> I. c) = (if I={} then SKIP else c)"
 by (rule program_equalityI, auto)
 
 lemma JN_Join_distrib:
-     "(JN i:I. F i Join G i) = (JN i:I. F i)  Join  (JN i:I. G i)"
+     "(\<Squnion>i \<in> I. F i Join G i) = (\<Squnion>i \<in> I. F i)  Join  (\<Squnion>i \<in> I. G i)"
 by (auto intro!: program_equalityI)
 
 lemma JN_Join_miniscope:
-     "i : I ==> (JN i:I. F i Join G) = ((JN i:I. F i) Join G)"
+     "i \<in> I ==> (\<Squnion>i \<in> I. F i Join G) = ((\<Squnion>i \<in> I. F i) Join G)"
 by (auto simp add: JN_Join_distrib JN_constant)
 
 (*Used to prove guarantees_JN_I*)
-lemma JN_Join_diff: "i: I ==> F i Join JOIN (I - {i}) F = JOIN I F"
+lemma JN_Join_diff: "i \<in> I ==> F i Join JOIN (I - {i}) F = JOIN I F"
 apply (unfold JOIN_def Join_def)
 apply (rule program_equalityI, auto)
 done
@@ -185,19 +185,19 @@ done
 
 subsection{*Safety: co, stable, FP*}
 
-(*Fails if I={} because it collapses to SKIP : A co B, i.e. to A<=B.  So an
-  alternative precondition is A<=B, but most proofs using this rule require
+(*Fails if I={} because it collapses to SKIP \<in> A co B, i.e. to A \<subseteq> B.  So an
+  alternative precondition is A \<subseteq> B, but most proofs using this rule require
   I to be nonempty for other reasons anyway.*)
 lemma JN_constrains: 
-    "i : I ==> (JN i:I. F i) : A co B = (ALL i:I. F i : A co B)"
+    "i \<in> I ==> (\<Squnion>i \<in> I. F i) \<in> A co B = (\<forall>i \<in> I. F i \<in> A co B)"
 by (simp add: constrains_def JOIN_def, blast)
 
 lemma Join_constrains [simp]:
-     "(F Join G : A co B) = (F : A co B & G : A co B)"
+     "(F Join G \<in> A co B) = (F \<in> A co B & G \<in> A co B)"
 by (auto simp add: constrains_def Join_def)
 
 lemma Join_unless [simp]:
-     "(F Join G : A unless B) = (F : A unless B & G : A unless B)"
+     "(F Join G \<in> A unless B) = (F \<in> A unless B & G \<in> A unless B)"
 by (simp add: Join_constrains unless_def)
 
 (*Analogous weak versions FAIL; see Misra [1994] 5.4.1, Substitution Axiom.
@@ -206,100 +206,100 @@ by (simp add: Join_constrains unless_def)
 
 
 lemma Join_constrains_weaken:
-     "[| F : A co A';  G : B co B' |]  
-      ==> F Join G : (A Int B) co (A' Un B')"
+     "[| F \<in> A co A';  G \<in> B co B' |]  
+      ==> F Join G \<in> (A \<inter> B) co (A' \<union> B')"
 by (simp, blast intro: constrains_weaken)
 
-(*If I={}, it degenerates to SKIP : UNIV co {}, which is false.*)
+(*If I={}, it degenerates to SKIP \<in> UNIV co {}, which is false.*)
 lemma JN_constrains_weaken:
-     "[| ALL i:I. F i : A i co A' i;  i: I |]  
-      ==> (JN i:I. F i) : (INT i:I. A i) co (UN i:I. A' i)"
+     "[| \<forall>i \<in> I. F i \<in> A i co A' i;  i \<in> I |]  
+      ==> (\<Squnion>i \<in> I. F i) \<in> (\<Inter>i \<in> I. A i) co (\<Union>i \<in> I. A' i)"
 apply (simp (no_asm_simp) add: JN_constrains)
 apply (blast intro: constrains_weaken)
 done
 
-lemma JN_stable: "(JN i:I. F i) : stable A = (ALL i:I. F i : stable A)"
+lemma JN_stable: "(\<Squnion>i \<in> I. F i) \<in> stable A = (\<forall>i \<in> I. F i \<in> stable A)"
 by (simp add: stable_def constrains_def JOIN_def)
 
 lemma invariant_JN_I:
-     "[| !!i. i:I ==> F i : invariant A;  i : I |]   
-       ==> (JN i:I. F i) : invariant A"
+     "[| !!i. i \<in> I ==> F i \<in> invariant A;  i \<in> I |]   
+       ==> (\<Squnion>i \<in> I. F i) \<in> invariant A"
 by (simp add: invariant_def JN_stable, blast)
 
 lemma Join_stable [simp]:
-     "(F Join G : stable A) =  
-      (F : stable A & G : stable A)"
+     "(F Join G \<in> stable A) =  
+      (F \<in> stable A & G \<in> stable A)"
 by (simp add: stable_def)
 
 lemma Join_increasing [simp]:
-     "(F Join G : increasing f) =  
-      (F : increasing f & G : increasing f)"
+     "(F Join G \<in> increasing f) =  
+      (F \<in> increasing f & G \<in> increasing f)"
 by (simp add: increasing_def Join_stable, blast)
 
 lemma invariant_JoinI:
-     "[| F : invariant A; G : invariant A |]   
-      ==> F Join G : invariant A"
+     "[| F \<in> invariant A; G \<in> invariant A |]   
+      ==> F Join G \<in> invariant A"
 by (simp add: invariant_def, blast)
 
-lemma FP_JN: "FP (JN i:I. F i) = (INT i:I. FP (F i))"
+lemma FP_JN: "FP (\<Squnion>i \<in> I. F i) = (\<Inter>i \<in> I. FP (F i))"
 by (simp add: FP_def JN_stable INTER_def)
 
 
 subsection{*Progress: transient, ensures*}
 
 lemma JN_transient:
-     "i : I ==>  
-    (JN i:I. F i) : transient A = (EX i:I. F i : transient A)"
+     "i \<in> I ==>  
+    (\<Squnion>i \<in> I. F i) \<in> transient A = (\<exists>i \<in> I. F i \<in> transient A)"
 by (auto simp add: transient_def JOIN_def)
 
 lemma Join_transient [simp]:
-     "F Join G : transient A =  
-      (F : transient A | G : transient A)"
+     "F Join G \<in> transient A =  
+      (F \<in> transient A | G \<in> transient A)"
 by (auto simp add: bex_Un transient_def Join_def)
 
-lemma Join_transient_I1: "F : transient A ==> F Join G : transient A"
+lemma Join_transient_I1: "F \<in> transient A ==> F Join G \<in> transient A"
 by (simp add: Join_transient)
 
-lemma Join_transient_I2: "G : transient A ==> F Join G : transient A"
+lemma Join_transient_I2: "G \<in> transient A ==> F Join G \<in> transient A"
 by (simp add: Join_transient)
 
-(*If I={} it degenerates to (SKIP : A ensures B) = False, i.e. to ~(A<=B) *)
+(*If I={} it degenerates to (SKIP \<in> A ensures B) = False, i.e. to ~(A \<subseteq> B) *)
 lemma JN_ensures:
-     "i : I ==>  
-      (JN i:I. F i) : A ensures B =  
-      ((ALL i:I. F i : (A-B) co (A Un B)) & (EX i:I. F i : A ensures B))"
+     "i \<in> I ==>  
+      (\<Squnion>i \<in> I. F i) \<in> A ensures B =  
+      ((\<forall>i \<in> I. F i \<in> (A-B) co (A \<union> B)) & (\<exists>i \<in> I. F i \<in> A ensures B))"
 by (auto simp add: ensures_def JN_constrains JN_transient)
 
 lemma Join_ensures: 
-     "F Join G : A ensures B =      
-      (F : (A-B) co (A Un B) & G : (A-B) co (A Un B) &  
-       (F : transient (A-B) | G : transient (A-B)))"
+     "F Join G \<in> A ensures B =      
+      (F \<in> (A-B) co (A \<union> B) & G \<in> (A-B) co (A \<union> B) &  
+       (F \<in> transient (A-B) | G \<in> transient (A-B)))"
 by (auto simp add: ensures_def Join_transient)
 
 lemma stable_Join_constrains: 
-    "[| F : stable A;  G : A co A' |]  
-     ==> F Join G : A co A'"
+    "[| F \<in> stable A;  G \<in> A co A' |]  
+     ==> F Join G \<in> A co A'"
 apply (unfold stable_def constrains_def Join_def)
 apply (simp add: ball_Un, blast)
 done
 
-(*Premise for G cannot use Always because  F: Stable A  is weaker than
-  G : stable A *)
+(*Premise for G cannot use Always because  F \<in> Stable A  is weaker than
+  G \<in> stable A *)
 lemma stable_Join_Always1:
-     "[| F : stable A;  G : invariant A |] ==> F Join G : Always A"
+     "[| F \<in> stable A;  G \<in> invariant A |] ==> F Join G \<in> Always A"
 apply (simp (no_asm_use) add: Always_def invariant_def Stable_eq_stable)
 apply (force intro: stable_Int)
 done
 
 (*As above, but exchanging the roles of F and G*)
 lemma stable_Join_Always2:
-     "[| F : invariant A;  G : stable A |] ==> F Join G : Always A"
+     "[| F \<in> invariant A;  G \<in> stable A |] ==> F Join G \<in> Always A"
 apply (subst Join_commute)
 apply (blast intro: stable_Join_Always1)
 done
 
 lemma stable_Join_ensures1:
-     "[| F : stable A;  G : A ensures B |] ==> F Join G : A ensures B"
+     "[| F \<in> stable A;  G \<in> A ensures B |] ==> F Join G \<in> A ensures B"
 apply (simp (no_asm_simp) add: Join_ensures)
 apply (simp add: stable_def ensures_def)
 apply (erule constrains_weaken, auto)
@@ -307,7 +307,7 @@ done
 
 (*As above, but exchanging the roles of F and G*)
 lemma stable_Join_ensures2:
-     "[| F : A ensures B;  G : stable A |] ==> F Join G : A ensures B"
+     "[| F \<in> A ensures B;  G \<in> stable A |] ==> F Join G \<in> A ensures B"
 apply (subst Join_commute)
 apply (blast intro: stable_Join_ensures1)
 done
@@ -344,16 +344,16 @@ by (auto simp add: ok_def)
 lemma ok_Join_commute_I: "[| F ok G; (F Join G) ok H |] ==> F ok (G Join H)"
 by (auto simp add: ok_def)
 
-lemma ok_JN_iff1 [iff]: "F ok (JOIN I G) = (ALL i:I. F ok G i)"
+lemma ok_JN_iff1 [iff]: "F ok (JOIN I G) = (\<forall>i \<in> I. F ok G i)"
 by (auto simp add: ok_def)
 
-lemma ok_JN_iff2 [iff]: "(JOIN I G) ok F =  (ALL i:I. G i ok F)"
+lemma ok_JN_iff2 [iff]: "(JOIN I G) ok F =  (\<forall>i \<in> I. G i ok F)"
 by (auto simp add: ok_def)
 
-lemma OK_iff_ok: "OK I F = (ALL i: I. ALL j: I-{i}. (F i) ok (F j))"
+lemma OK_iff_ok: "OK I F = (\<forall>i \<in> I. \<forall>j \<in> I-{i}. (F i) ok (F j))"
 by (auto simp add: ok_def OK_def)
 
-lemma OK_imp_ok: "[| OK I F; i: I; j: I; i ~= j|] ==> (F i) ok (F j)"
+lemma OK_imp_ok: "[| OK I F; i \<in> I; j \<in> I; i \<noteq> j|] ==> (F i) ok (F j)"
 by (auto simp add: OK_iff_ok)
 
 
@@ -362,27 +362,27 @@ subsection{*Allowed*}
 lemma Allowed_SKIP [simp]: "Allowed SKIP = UNIV"
 by (auto simp add: Allowed_def)
 
-lemma Allowed_Join [simp]: "Allowed (F Join G) = Allowed F Int Allowed G"
+lemma Allowed_Join [simp]: "Allowed (F Join G) = Allowed F \<inter> Allowed G"
 by (auto simp add: Allowed_def)
 
-lemma Allowed_JN [simp]: "Allowed (JOIN I F) = (INT i:I. Allowed (F i))"
+lemma Allowed_JN [simp]: "Allowed (JOIN I F) = (\<Inter>i \<in> I. Allowed (F i))"
 by (auto simp add: Allowed_def)
 
-lemma ok_iff_Allowed: "F ok G = (F : Allowed G & G : Allowed F)"
+lemma ok_iff_Allowed: "F ok G = (F \<in> Allowed G & G \<in> Allowed F)"
 by (simp add: ok_def Allowed_def)
 
-lemma OK_iff_Allowed: "OK I F = (ALL i: I. ALL j: I-{i}. F i : Allowed(F j))"
+lemma OK_iff_Allowed: "OK I F = (\<forall>i \<in> I. \<forall>j \<in> I-{i}. F i \<in> Allowed(F j))"
 by (auto simp add: OK_iff_ok ok_iff_Allowed)
 
 subsection{*@{text safety_prop}, for reasoning about
  given instances of "ok"*}
 
 lemma safety_prop_Acts_iff:
-     "safety_prop X ==> (Acts G <= insert Id (UNION X Acts)) = (G : X)"
+     "safety_prop X ==> (Acts G \<subseteq> insert Id (UNION X Acts)) = (G \<in> X)"
 by (auto simp add: safety_prop_def)
 
 lemma safety_prop_AllowedActs_iff_Allowed:
-     "safety_prop X ==> (UNION X Acts <= AllowedActs F) = (X <= Allowed F)"
+     "safety_prop X ==> (UNION X Acts \<subseteq> AllowedActs F) = (X \<subseteq> Allowed F)"
 by (auto simp add: Allowed_def safety_prop_Acts_iff [symmetric])
 
 lemma Allowed_eq:
@@ -395,27 +395,27 @@ lemma def_prg_Allowed:
 by (simp add: Allowed_eq)
 
 (*For safety_prop to hold, the property must be satisfiable!*)
-lemma safety_prop_constrains [iff]: "safety_prop (A co B) = (A <= B)"
+lemma safety_prop_constrains [iff]: "safety_prop (A co B) = (A \<subseteq> B)"
 by (simp add: safety_prop_def constrains_def, blast)
 
 lemma safety_prop_stable [iff]: "safety_prop (stable A)"
 by (simp add: stable_def)
 
 lemma safety_prop_Int [simp]:
-     "[| safety_prop X; safety_prop Y |] ==> safety_prop (X Int Y)"
+     "[| safety_prop X; safety_prop Y |] ==> safety_prop (X \<inter> Y)"
 by (simp add: safety_prop_def, blast)
 
 lemma safety_prop_INTER1 [simp]:
-     "(!!i. safety_prop (X i)) ==> safety_prop (INT i. X i)"
+     "(!!i. safety_prop (X i)) ==> safety_prop (\<Inter>i. X i)"
 by (auto simp add: safety_prop_def, blast)
 							       
 lemma safety_prop_INTER [simp]:
-     "(!!i. i:I ==> safety_prop (X i)) ==> safety_prop (INT i:I. X i)"
+     "(!!i. i \<in> I ==> safety_prop (X i)) ==> safety_prop (\<Inter>i \<in> I. X i)"
 by (auto simp add: safety_prop_def, blast)
 
 lemma def_UNION_ok_iff:
      "[| F == mk_program(init,acts,UNION X Acts); safety_prop X |]  
-      ==> F ok G = (G : X & acts <= AllowedActs G)"
+      ==> F ok G = (G \<in> X & acts \<subseteq> AllowedActs G)"
 by (auto simp add: ok_def safety_prop_Acts_iff)
 
 end
