src/HOL/UNITY/WFair.thy
@@ -17,10 +17,10 @@ constdefs
   (*This definition specifies weak fairness.  The rest of the theory
     is generic to all forms of fairness.*)
   transient :: "'a set => 'a program set"
-    "transient A == {F. EX act: Acts F. A <= Domain act & act``A <= -A}"
+    "transient A == {F. \<exists>act\<in>Acts F. A \<subseteq> Domain act & act``A \<subseteq> -A}"
 
   ensures :: "['a set, 'a set] => 'a program set"       (infixl "ensures" 60)
-    "A ensures B == (A-B co A Un B) Int transient (A-B)"
+    "A ensures B == (A-B co A \<union> B) \<inter> transient (A-B)"
 
 
 consts
@@ -32,22 +32,22 @@ consts
 inductive "leads F"
   intros 
 
-    Basis:  "F : A ensures B ==> (A,B) : leads F"
+    Basis:  "F \<in> A ensures B ==> (A,B) \<in> leads F"
 
-    Trans:  "[| (A,B) : leads F;  (B,C) : leads F |] ==> (A,C) : leads F"
+    Trans:  "[| (A,B) \<in> leads F;  (B,C) \<in> leads F |] ==> (A,C) \<in> leads F"
 
-    Union:  "ALL A: S. (A,B) : leads F ==> (Union S, B) : leads F"
+    Union:  "\<forall>A \<in> S. (A,B) \<in> leads F ==> (Union S, B) \<in> leads F"
 
 
 constdefs
 
   (*visible version of the LEADS-TO relation*)
   leadsTo :: "['a set, 'a set] => 'a program set"    (infixl "leadsTo" 60)
-    "A leadsTo B == {F. (A,B) : leads F}"
+    "A leadsTo B == {F. (A,B) \<in> leads F}"
   
   (*wlt F B is the largest set that leads to B*)
   wlt :: "['a program, 'a set] => 'a set"
-    "wlt F B == Union {A. F: A leadsTo B}"
+    "wlt F B == Union {A. F \<in> A leadsTo B}"
 
 syntax (xsymbols)
   "op leadsTo" :: "['a set, 'a set] => 'a program set" (infixl "\<longmapsto>" 60)
@@ -56,22 +56,22 @@ syntax (xsymbols)
 subsection{*transient*}
 
 lemma stable_transient_empty: 
-    "[| F : stable A; F : transient A |] ==> A = {}"
+    "[| F \<in> stable A; F \<in> transient A |] ==> A = {}"
 by (unfold stable_def constrains_def transient_def, blast)
 
 lemma transient_strengthen: 
-    "[| F : transient A; B<=A |] ==> F : transient B"
+    "[| F \<in> transient A; B \<subseteq> A |] ==> F \<in> transient B"
 apply (unfold transient_def, clarify)
 apply (blast intro!: rev_bexI)
 done
 
 lemma transientI: 
-    "[| act: Acts F;  A <= Domain act;  act``A <= -A |] ==> F : transient A"
+    "[| act: Acts F;  A \<subseteq> Domain act;  act``A \<subseteq> -A |] ==> F \<in> transient A"
 by (unfold transient_def, blast)
 
 lemma transientE: 
-    "[| F : transient A;   
-        !!act. [| act: Acts F;  A <= Domain act;  act``A <= -A |] ==> P |]  
+    "[| F \<in> transient A;   
+        !!act. [| act: Acts F;  A \<subseteq> Domain act;  act``A \<subseteq> -A |] ==> P |]  
      ==> P"
 by (unfold transient_def, blast)
 
@@ -85,23 +85,23 @@ by (unfold transient_def, auto)
 subsection{*ensures*}
 
 lemma ensuresI: 
-    "[| F : (A-B) co (A Un B); F : transient (A-B) |] ==> F : A ensures B"
+    "[| F \<in> (A-B) co (A \<union> B); F \<in> transient (A-B) |] ==> F \<in> A ensures B"
 by (unfold ensures_def, blast)
 
 lemma ensuresD: 
-    "F : A ensures B ==> F : (A-B) co (A Un B) & F : transient (A-B)"
+    "F \<in> A ensures B ==> F \<in> (A-B) co (A \<union> B) & F \<in> transient (A-B)"
 by (unfold ensures_def, blast)
 
 lemma ensures_weaken_R: 
-    "[| F : A ensures A'; A'<=B' |] ==> F : A ensures B'"
+    "[| F \<in> A ensures A'; A'<=B' |] ==> F \<in> A ensures B'"
 apply (unfold ensures_def)
 apply (blast intro: constrains_weaken transient_strengthen)
 done
 
 (*The L-version (precondition strengthening) fails, but we have this*)
 lemma stable_ensures_Int: 
-    "[| F : stable C;  F : A ensures B |]    
-    ==> F : (C Int A) ensures (C Int B)"
+    "[| F \<in> stable C;  F \<in> A ensures B |]    
+    ==> F \<in> (C \<inter> A) ensures (C \<inter> B)"
 apply (unfold ensures_def)
 apply (auto simp add: ensures_def Int_Un_distrib [symmetric] Diff_Int_distrib [symmetric])
 prefer 2 apply (blast intro: transient_strengthen)
@@ -109,78 +109,78 @@ apply (blast intro: stable_constrains_Int constrains_weaken)
 done
 
 lemma stable_transient_ensures:
-     "[| F : stable A;  F : transient C;  A <= B Un C |] ==> F : A ensures B"
+     "[| F \<in> stable A;  F \<in> transient C;  A \<subseteq> B \<union> C |] ==> F \<in> A ensures B"
 apply (simp add: ensures_def stable_def)
 apply (blast intro: constrains_weaken transient_strengthen)
 done
 
-lemma ensures_eq: "(A ensures B) = (A unless B) Int transient (A-B)"
+lemma ensures_eq: "(A ensures B) = (A unless B) \<inter> transient (A-B)"
 by (simp (no_asm) add: ensures_def unless_def)
 
 
 subsection{*leadsTo*}
 
-lemma leadsTo_Basis [intro]: "F : A ensures B ==> F : A leadsTo B"
+lemma leadsTo_Basis [intro]: "F \<in> A ensures B ==> F \<in> A leadsTo B"
 apply (unfold leadsTo_def)
 apply (blast intro: leads.Basis)
 done
 
 lemma leadsTo_Trans: 
-     "[| F : A leadsTo B;  F : B leadsTo C |] ==> F : A leadsTo C"
+     "[| F \<in> A leadsTo B;  F \<in> B leadsTo C |] ==> F \<in> A leadsTo C"
 apply (unfold leadsTo_def)
 apply (blast intro: leads.Trans)
 done
 
-lemma transient_imp_leadsTo: "F : transient A ==> F : A leadsTo (-A)"
+lemma transient_imp_leadsTo: "F \<in> transient A ==> F \<in> A leadsTo (-A)"
 by (simp (no_asm_simp) add: leadsTo_Basis ensuresI Compl_partition)
 
 (*Useful with cancellation, disjunction*)
-lemma leadsTo_Un_duplicate: "F : A leadsTo (A' Un A') ==> F : A leadsTo A'"
+lemma leadsTo_Un_duplicate: "F \<in> A leadsTo (A' \<union> A') ==> F \<in> A leadsTo A'"
 by (simp add: Un_ac)
 
 lemma leadsTo_Un_duplicate2:
-     "F : A leadsTo (A' Un C Un C) ==> F : A leadsTo (A' Un C)"
+     "F \<in> A leadsTo (A' \<union> C \<union> C) ==> F \<in> A leadsTo (A' \<union> C)"
 by (simp add: Un_ac)
 
 (*The Union introduction rule as we should have liked to state it*)
 lemma leadsTo_Union: 
-    "(!!A. A : S ==> F : A leadsTo B) ==> F : (Union S) leadsTo B"
+    "(!!A. A \<in> S ==> F \<in> A leadsTo B) ==> F \<in> (Union S) leadsTo B"
 apply (unfold leadsTo_def)
 apply (blast intro: leads.Union)
 done
 
 lemma leadsTo_Union_Int: 
- "(!!A. A : S ==> F : (A Int C) leadsTo B) ==> F : (Union S Int C) leadsTo B"
+ "(!!A. A \<in> S ==> F \<in> (A \<inter> C) leadsTo B) ==> F \<in> (Union S \<inter> C) leadsTo B"
 apply (unfold leadsTo_def)
 apply (simp only: Int_Union_Union)
 apply (blast intro: leads.Union)
 done
 
 lemma leadsTo_UN: 
-    "(!!i. i : I ==> F : (A i) leadsTo B) ==> F : (UN i:I. A i) leadsTo B"
+    "(!!i. i \<in> I ==> F \<in> (A i) leadsTo B) ==> F \<in> (\<Union>i \<in> I. A i) leadsTo B"
 apply (subst Union_image_eq [symmetric])
 apply (blast intro: leadsTo_Union)
 done
 
 (*Binary union introduction rule*)
 lemma leadsTo_Un:
-     "[| F : A leadsTo C; F : B leadsTo C |] ==> F : (A Un B) leadsTo C"
+     "[| F \<in> A leadsTo C; F \<in> B leadsTo C |] ==> F \<in> (A \<union> B) leadsTo C"
 apply (subst Un_eq_Union)
 apply (blast intro: leadsTo_Union)
 done
 
 lemma single_leadsTo_I: 
-     "(!!x. x : A ==> F : {x} leadsTo B) ==> F : A leadsTo B"
+     "(!!x. x \<in> A ==> F \<in> {x} leadsTo B) ==> F \<in> A leadsTo B"
 by (subst UN_singleton [symmetric], rule leadsTo_UN, blast)
 
 
 (*The INDUCTION rule as we should have liked to state it*)
 lemma leadsTo_induct: 
-  "[| F : za leadsTo zb;   
-      !!A B. F : A ensures B ==> P A B;  
-      !!A B C. [| F : A leadsTo B; P A B; F : B leadsTo C; P B C |]  
+  "[| F \<in> za leadsTo zb;   
+      !!A B. F \<in> A ensures B ==> P A B;  
+      !!A B C. [| F \<in> A leadsTo B; P A B; F \<in> B leadsTo C; P B C |]  
                ==> P A C;  
-      !!B S. ALL A:S. F : A leadsTo B & P A B ==> P (Union S) B  
+      !!B S. \<forall>A \<in> S. F \<in> A leadsTo B & P A B ==> P (Union S) B  
    |] ==> P za zb"
 apply (unfold leadsTo_def)
 apply (drule CollectD, erule leads.induct)
@@ -188,7 +188,7 @@ apply (blast+)
 done
 
 
-lemma subset_imp_ensures: "A<=B ==> F : A ensures B"
+lemma subset_imp_ensures: "A \<subseteq> B ==> F \<in> A ensures B"
 by (unfold ensures_def constrains_def transient_def, blast)
 
 lemmas subset_imp_leadsTo = subset_imp_ensures [THEN leadsTo_Basis, standard]
@@ -205,10 +205,10 @@ lemmas leadsTo_UNIV = subset_UNIV [THEN subset_imp_leadsTo, standard, simp]
 
 (*Lemma is the weak version: can't see how to do it in one step*)
 lemma leadsTo_induct_pre_lemma: 
-  "[| F : za leadsTo zb;   
+  "[| F \<in> za leadsTo zb;   
       P zb;  
-      !!A B. [| F : A ensures B;  P B |] ==> P A;  
-      !!S. ALL A:S. P A ==> P (Union S)  
+      !!A B. [| F \<in> A ensures B;  P B |] ==> P A;  
+      !!S. \<forall>A \<in> S. P A ==> P (Union S)  
    |] ==> P za"
 (*by induction on this formula*)
 apply (subgoal_tac "P zb --> P za")
@@ -219,12 +219,12 @@ apply (blast+)
 done
 
 lemma leadsTo_induct_pre: 
-  "[| F : za leadsTo zb;   
+  "[| F \<in> za leadsTo zb;   
       P zb;  
-      !!A B. [| F : A ensures B;  F : B leadsTo zb;  P B |] ==> P A;  
-      !!S. ALL A:S. F : A leadsTo zb & P A ==> P (Union S)  
+      !!A B. [| F \<in> A ensures B;  F \<in> B leadsTo zb;  P B |] ==> P A;  
+      !!S. \<forall>A \<in> S. F \<in> A leadsTo zb & P A ==> P (Union S)  
    |] ==> P za"
-apply (subgoal_tac "F : za leadsTo zb & P za")
+apply (subgoal_tac "F \<in> za leadsTo zb & P za")
 apply (erule conjunct2)
 apply (erule leadsTo_induct_pre_lemma)
 prefer 3 apply (blast intro: leadsTo_Union)
@@ -233,76 +233,76 @@ apply (blast intro: leadsTo_refl)
 done
 
 
-lemma leadsTo_weaken_R: "[| F : A leadsTo A'; A'<=B' |] ==> F : A leadsTo B'"
+lemma leadsTo_weaken_R: "[| F \<in> A leadsTo A'; A'<=B' |] ==> F \<in> A leadsTo B'"
 by (blast intro: subset_imp_leadsTo leadsTo_Trans)
 
 lemma leadsTo_weaken_L [rule_format]:
-     "[| F : A leadsTo A'; B<=A |] ==> F : B leadsTo A'"
+     "[| F \<in> A leadsTo A'; B \<subseteq> A |] ==> F \<in> B leadsTo A'"
 by (blast intro: leadsTo_Trans subset_imp_leadsTo)
 
 (*Distributes over binary unions*)
 lemma leadsTo_Un_distrib:
-     "F : (A Un B) leadsTo C  =  (F : A leadsTo C & F : B leadsTo C)"
+     "F \<in> (A \<union> B) leadsTo C  =  (F \<in> A leadsTo C & F \<in> B leadsTo C)"
 by (blast intro: leadsTo_Un leadsTo_weaken_L)
 
 lemma leadsTo_UN_distrib:
-     "F : (UN i:I. A i) leadsTo B  =  (ALL i : I. F : (A i) leadsTo B)"
+     "F \<in> (\<Union>i \<in> I. A i) leadsTo B  =  (\<forall>i \<in> I. F \<in> (A i) leadsTo B)"
 by (blast intro: leadsTo_UN leadsTo_weaken_L)
 
 lemma leadsTo_Union_distrib:
-     "F : (Union S) leadsTo B  =  (ALL A : S. F : A leadsTo B)"
+     "F \<in> (Union S) leadsTo B  =  (\<forall>A \<in> S. F \<in> A leadsTo B)"
 by (blast intro: leadsTo_Union leadsTo_weaken_L)
 
 
 lemma leadsTo_weaken:
-     "[| F : A leadsTo A'; B<=A; A'<=B' |] ==> F : B leadsTo B'"
+     "[| F \<in> A leadsTo A'; B \<subseteq> A; A'<=B' |] ==> F \<in> B leadsTo B'"
 by (blast intro: leadsTo_weaken_R leadsTo_weaken_L leadsTo_Trans)
 
 
 (*Set difference: maybe combine with leadsTo_weaken_L?*)
 lemma leadsTo_Diff:
-     "[| F : (A-B) leadsTo C; F : B leadsTo C |]   ==> F : A leadsTo C"
+     "[| F \<in> (A-B) leadsTo C; F \<in> B leadsTo C |]   ==> F \<in> A leadsTo C"
 by (blast intro: leadsTo_Un leadsTo_weaken)
 
 lemma leadsTo_UN_UN:
-   "(!! i. i:I ==> F : (A i) leadsTo (A' i))  
-    ==> F : (UN i:I. A i) leadsTo (UN i:I. A' i)"
+   "(!! i. i \<in> I ==> F \<in> (A i) leadsTo (A' i))  
+    ==> F \<in> (\<Union>i \<in> I. A i) leadsTo (\<Union>i \<in> I. A' i)"
 apply (simp only: Union_image_eq [symmetric])
 apply (blast intro: leadsTo_Union leadsTo_weaken_R)
 done
 
 (*Binary union version*)
 lemma leadsTo_Un_Un:
-     "[| F : A leadsTo A'; F : B leadsTo B' |]  
-      ==> F : (A Un B) leadsTo (A' Un B')"
+     "[| F \<in> A leadsTo A'; F \<in> B leadsTo B' |]  
+      ==> F \<in> (A \<union> B) leadsTo (A' \<union> B')"
 by (blast intro: leadsTo_Un leadsTo_weaken_R)
 
 
 (** The cancellation law **)
 
 lemma leadsTo_cancel2:
-     "[| F : A leadsTo (A' Un B); F : B leadsTo B' |]  
-      ==> F : A leadsTo (A' Un B')"
+     "[| F \<in> A leadsTo (A' \<union> B); F \<in> B leadsTo B' |]  
+      ==> F \<in> A leadsTo (A' \<union> B')"
 by (blast intro: leadsTo_Un_Un subset_imp_leadsTo leadsTo_Trans)
 
 lemma leadsTo_cancel_Diff2:
-     "[| F : A leadsTo (A' Un B); F : (B-A') leadsTo B' |]  
-      ==> F : A leadsTo (A' Un B')"
+     "[| F \<in> A leadsTo (A' \<union> B); F \<in> (B-A') leadsTo B' |]  
+      ==> F \<in> A leadsTo (A' \<union> B')"
 apply (rule leadsTo_cancel2)
 prefer 2 apply assumption
 apply (simp_all (no_asm_simp))
 done
 
 lemma leadsTo_cancel1:
-     "[| F : A leadsTo (B Un A'); F : B leadsTo B' |]  
-    ==> F : A leadsTo (B' Un A')"
+     "[| F \<in> A leadsTo (B \<union> A'); F \<in> B leadsTo B' |]  
+    ==> F \<in> A leadsTo (B' \<union> A')"
 apply (simp add: Un_commute)
 apply (blast intro!: leadsTo_cancel2)
 done
 
 lemma leadsTo_cancel_Diff1:
-     "[| F : A leadsTo (B Un A'); F : (B-A') leadsTo B' |]  
-    ==> F : A leadsTo (B' Un A')"
+     "[| F \<in> A leadsTo (B \<union> A'); F \<in> (B-A') leadsTo B' |]  
+    ==> F \<in> A leadsTo (B' \<union> A')"
 apply (rule leadsTo_cancel1)
 prefer 2 apply assumption
 apply (simp_all (no_asm_simp))
@@ -312,7 +312,7 @@ done
 
 (** The impossibility law **)
 
-lemma leadsTo_empty: "F : A leadsTo {} ==> A={}"
+lemma leadsTo_empty: "F \<in> A leadsTo {} ==> A={}"
 apply (erule leadsTo_induct_pre)
 apply (simp_all add: ensures_def constrains_def transient_def, blast)
 done
@@ -322,8 +322,8 @@ done
 
 (*Special case of PSP: Misra's "stable conjunction"*)
 lemma psp_stable: 
-   "[| F : A leadsTo A'; F : stable B |]  
-    ==> F : (A Int B) leadsTo (A' Int B)"
+   "[| F \<in> A leadsTo A'; F \<in> stable B |]  
+    ==> F \<in> (A \<inter> B) leadsTo (A' \<inter> B)"
 apply (unfold stable_def)
 apply (erule leadsTo_induct)
 prefer 3 apply (blast intro: leadsTo_Union_Int)
@@ -334,19 +334,19 @@ apply (blast intro: transient_strengthen constrains_Int)
 done
 
 lemma psp_stable2: 
-   "[| F : A leadsTo A'; F : stable B |] ==> F : (B Int A) leadsTo (B Int A')"
+   "[| F \<in> A leadsTo A'; F \<in> stable B |] ==> F \<in> (B \<inter> A) leadsTo (B \<inter> A')"
 by (simp add: psp_stable Int_ac)
 
 lemma psp_ensures: 
-   "[| F : A ensures A'; F : B co B' |]  
-    ==> F : (A Int B') ensures ((A' Int B) Un (B' - B))"
+   "[| F \<in> A ensures A'; F \<in> B co B' |]  
+    ==> F \<in> (A \<inter> B') ensures ((A' \<inter> B) \<union> (B' - B))"
 apply (unfold ensures_def constrains_def, clarify) (*speeds up the proof*)
 apply (blast intro: transient_strengthen)
 done
 
 lemma psp:
-     "[| F : A leadsTo A'; F : B co B' |]  
-      ==> F : (A Int B') leadsTo ((A' Int B) Un (B' - B))"
+     "[| F \<in> A leadsTo A'; F \<in> B co B' |]  
+      ==> F \<in> (A \<inter> B') leadsTo ((A' \<inter> B) \<union> (B' - B))"
 apply (erule leadsTo_induct)
   prefer 3 apply (blast intro: leadsTo_Union_Int)
  txt{*Basis case*}
@@ -359,13 +359,13 @@ apply (blast intro: leadsTo_weaken_L dest: constrains_imp_subset)
 done
 
 lemma psp2:
-     "[| F : A leadsTo A'; F : B co B' |]  
-    ==> F : (B' Int A) leadsTo ((B Int A') Un (B' - B))"
+     "[| F \<in> A leadsTo A'; F \<in> B co B' |]  
+    ==> F \<in> (B' \<inter> A) leadsTo ((B \<inter> A') \<union> (B' - B))"
 by (simp (no_asm_simp) add: psp Int_ac)
 
 lemma psp_unless: 
-   "[| F : A leadsTo A';  F : B unless B' |]  
-    ==> F : (A Int B) leadsTo ((A' Int B) Un B')"
+   "[| F \<in> A leadsTo A';  F \<in> B unless B' |]  
+    ==> F \<in> (A \<inter> B) leadsTo ((A' \<inter> B) \<union> B')"
 
 apply (unfold unless_def)
 apply (drule psp, assumption)
@@ -379,11 +379,11 @@ subsection{*Proving the induction rules*}
 
 lemma leadsTo_wf_induct_lemma:
      "[| wf r;      
-         ALL m. F : (A Int f-`{m}) leadsTo                      
-                    ((A Int f-`(r^-1 `` {m})) Un B) |]  
-      ==> F : (A Int f-`{m}) leadsTo B"
+         \<forall>m. F \<in> (A \<inter> f-`{m}) leadsTo                      
+                    ((A \<inter> f-`(r^-1 `` {m})) \<union> B) |]  
+      ==> F \<in> (A \<inter> f-`{m}) leadsTo B"
 apply (erule_tac a = m in wf_induct)
-apply (subgoal_tac "F : (A Int (f -` (r^-1 `` {x}))) leadsTo B")
+apply (subgoal_tac "F \<in> (A \<inter> (f -` (r^-1 `` {x}))) leadsTo B")
  apply (blast intro: leadsTo_cancel1 leadsTo_Un_duplicate)
 apply (subst vimage_eq_UN)
 apply (simp only: UN_simps [symmetric])
@@ -394,9 +394,9 @@ done
 (** Meta or object quantifier ? **)
 lemma leadsTo_wf_induct:
      "[| wf r;      
-         ALL m. F : (A Int f-`{m}) leadsTo                      
-                    ((A Int f-`(r^-1 `` {m})) Un B) |]  
-      ==> F : A leadsTo B"
+         \<forall>m. F \<in> (A \<inter> f-`{m}) leadsTo                      
+                    ((A \<inter> f-`(r^-1 `` {m})) \<union> B) |]  
+      ==> F \<in> A leadsTo B"
 apply (rule_tac t = A in subst)
  defer 1
  apply (rule leadsTo_UN)
@@ -408,102 +408,102 @@ done
 
 lemma bounded_induct:
      "[| wf r;      
-         ALL m:I. F : (A Int f-`{m}) leadsTo                    
-                      ((A Int f-`(r^-1 `` {m})) Un B) |]  
-      ==> F : A leadsTo ((A - (f-`I)) Un B)"
+         \<forall>m \<in> I. F \<in> (A \<inter> f-`{m}) leadsTo                    
+                      ((A \<inter> f-`(r^-1 `` {m})) \<union> B) |]  
+      ==> F \<in> A leadsTo ((A - (f-`I)) \<union> B)"
 apply (erule leadsTo_wf_induct, safe)
-apply (case_tac "m:I")
+apply (case_tac "m \<in> I")
 apply (blast intro: leadsTo_weaken)
 apply (blast intro: subset_imp_leadsTo)
 done
 
 
-(*Alternative proof is via the lemma F : (A Int f-`(lessThan m)) leadsTo B*)
+(*Alternative proof is via the lemma F \<in> (A \<inter> f-`(lessThan m)) leadsTo B*)
 lemma lessThan_induct: 
-     "[| !!m::nat. F : (A Int f-`{m}) leadsTo ((A Int f-`{..m(}) Un B) |]  
-      ==> F : A leadsTo B"
+     "[| !!m::nat. F \<in> (A \<inter> f-`{m}) leadsTo ((A \<inter> f-`{..m(}) \<union> B) |]  
+      ==> F \<in> A leadsTo B"
 apply (rule wf_less_than [THEN leadsTo_wf_induct])
 apply (simp (no_asm_simp))
 apply blast
 done
 
 lemma lessThan_bounded_induct:
-     "!!l::nat. [| ALL m:(greaterThan l).     
-            F : (A Int f-`{m}) leadsTo ((A Int f-`(lessThan m)) Un B) |]  
-      ==> F : A leadsTo ((A Int (f-`(atMost l))) Un B)"
+     "!!l::nat. [| \<forall>m \<in> greaterThan l.     
+            F \<in> (A \<inter> f-`{m}) leadsTo ((A \<inter> f-`(lessThan m)) \<union> B) |]  
+      ==> F \<in> A leadsTo ((A \<inter> (f-`(atMost l))) \<union> B)"
 apply (simp only: Diff_eq [symmetric] vimage_Compl Compl_greaterThan [symmetric])
 apply (rule wf_less_than [THEN bounded_induct])
 apply (simp (no_asm_simp))
 done
 
 lemma greaterThan_bounded_induct:
-     "!!l::nat. [| ALL m:(lessThan l).     
-            F : (A Int f-`{m}) leadsTo ((A Int f-`(greaterThan m)) Un B) |]  
-      ==> F : A leadsTo ((A Int (f-`(atLeast l))) Un B)"
+     "(!!l::nat. \<forall>m \<in> lessThan l.     
+                 F \<in> (A \<inter> f-`{m}) leadsTo ((A \<inter> f-`(greaterThan m)) \<union> B))
+      ==> F \<in> A leadsTo ((A \<inter> (f-`(atLeast l))) \<union> B)"
 apply (rule_tac f = f and f1 = "%k. l - k" 
        in wf_less_than [THEN wf_inv_image, THEN leadsTo_wf_induct])
 apply (simp (no_asm) add: inv_image_def Image_singleton)
 apply clarify
 apply (case_tac "m<l")
-prefer 2 apply (blast intro: not_leE subset_imp_leadsTo)
-apply (blast intro: leadsTo_weaken_R diff_less_mono2)
+ apply (blast intro: leadsTo_weaken_R diff_less_mono2)
+apply (blast intro: not_leE subset_imp_leadsTo)
 done
 
 
 subsection{*wlt*}
 
 (*Misra's property W3*)
-lemma wlt_leadsTo: "F : (wlt F B) leadsTo B"
+lemma wlt_leadsTo: "F \<in> (wlt F B) leadsTo B"
 apply (unfold wlt_def)
 apply (blast intro!: leadsTo_Union)
 done
 
-lemma leadsTo_subset: "F : A leadsTo B ==> A <= wlt F B"
+lemma leadsTo_subset: "F \<in> A leadsTo B ==> A \<subseteq> wlt F B"
 apply (unfold wlt_def)
 apply (blast intro!: leadsTo_Union)
 done
 
 (*Misra's property W2*)
-lemma leadsTo_eq_subset_wlt: "F : A leadsTo B = (A <= wlt F B)"
+lemma leadsTo_eq_subset_wlt: "F \<in> A leadsTo B = (A \<subseteq> wlt F B)"
 by (blast intro!: leadsTo_subset wlt_leadsTo [THEN leadsTo_weaken_L])
 
 (*Misra's property W4*)
-lemma wlt_increasing: "B <= wlt F B"
+lemma wlt_increasing: "B \<subseteq> wlt F B"
 apply (simp (no_asm_simp) add: leadsTo_eq_subset_wlt [symmetric] subset_imp_leadsTo)
 done
 
 
 (*Used in the Trans case below*)
 lemma lemma1: 
-   "[| B <= A2;   
-       F : (A1 - B) co (A1 Un B);  
-       F : (A2 - C) co (A2 Un C) |]  
-    ==> F : (A1 Un A2 - C) co (A1 Un A2 Un C)"
+   "[| B \<subseteq> A2;   
+       F \<in> (A1 - B) co (A1 \<union> B);  
+       F \<in> (A2 - C) co (A2 \<union> C) |]  
+    ==> F \<in> (A1 \<union> A2 - C) co (A1 \<union> A2 \<union> C)"
 by (unfold constrains_def, clarify,  blast)
 
 (*Lemma (1,2,3) of Misra's draft book, Chapter 4, "Progress"*)
 lemma leadsTo_123:
-     "F : A leadsTo A'  
-      ==> EX B. A<=B & F : B leadsTo A' & F : (B-A') co (B Un A')"
+     "F \<in> A leadsTo A'  
+      ==> \<exists>B. A \<subseteq> B & F \<in> B leadsTo A' & F \<in> (B-A') co (B \<union> A')"
 apply (erule leadsTo_induct)
 (*Basis*)
 apply (blast dest: ensuresD)
 (*Trans*)
 apply clarify
-apply (rule_tac x = "Ba Un Bb" in exI)
+apply (rule_tac x = "Ba \<union> Bb" in exI)
 apply (blast intro: lemma1 leadsTo_Un_Un leadsTo_cancel1 leadsTo_Un_duplicate)
 (*Union*)
 apply (clarify dest!: ball_conj_distrib [THEN iffD1] bchoice)
-apply (rule_tac x = "UN A:S. f A" in exI)
+apply (rule_tac x = "\<Union>A \<in> S. f A" in exI)
 apply (auto intro: leadsTo_UN)
 (*Blast_tac says PROOF FAILED*)
-apply (rule_tac I1=S and A1="%i. f i - B" and A'1="%i. f i Un B" 
+apply (rule_tac I1=S and A1="%i. f i - B" and A'1="%i. f i \<union> B" 
        in constrains_UN [THEN constrains_weaken], auto) 
 done
 
 
 (*Misra's property W5*)
-lemma wlt_constrains_wlt: "F : (wlt F B - B) co (wlt F B)"
+lemma wlt_constrains_wlt: "F \<in> (wlt F B - B) co (wlt F B)"
 proof -
   from wlt_leadsTo [of F B, THEN leadsTo_123]
   show ?thesis
@@ -527,28 +527,28 @@ qed
 subsection{*Completion: Binary and General Finite versions*}
 
 lemma completion_lemma :
-     "[| W = wlt F (B' Un C);      
-       F : A leadsTo (A' Un C);  F : A' co (A' Un C);    
-       F : B leadsTo (B' Un C);  F : B' co (B' Un C) |]  
-    ==> F : (A Int B) leadsTo ((A' Int B') Un C)"
-apply (subgoal_tac "F : (W-C) co (W Un B' Un C) ")
+     "[| W = wlt F (B' \<union> C);      
+       F \<in> A leadsTo (A' \<union> C);  F \<in> A' co (A' \<union> C);    
+       F \<in> B leadsTo (B' \<union> C);  F \<in> B' co (B' \<union> C) |]  
+    ==> F \<in> (A \<inter> B) leadsTo ((A' \<inter> B') \<union> C)"
+apply (subgoal_tac "F \<in> (W-C) co (W \<union> B' \<union> C) ")
  prefer 2
  apply (blast intro: wlt_constrains_wlt [THEN [2] constrains_Un, 
                                          THEN constrains_weaken])
-apply (subgoal_tac "F : (W-C) co W")
+apply (subgoal_tac "F \<in> (W-C) co W")
  prefer 2
  apply (simp add: wlt_increasing Un_assoc Un_absorb2)
-apply (subgoal_tac "F : (A Int W - C) leadsTo (A' Int W Un C) ")
+apply (subgoal_tac "F \<in> (A \<inter> W - C) leadsTo (A' \<inter> W \<union> C) ")
  prefer 2 apply (blast intro: wlt_leadsTo psp [THEN leadsTo_weaken])
 (** LEVEL 6 **)
-apply (subgoal_tac "F : (A' Int W Un C) leadsTo (A' Int B' Un C) ")
+apply (subgoal_tac "F \<in> (A' \<inter> W \<union> C) leadsTo (A' \<inter> B' \<union> C) ")
  prefer 2
  apply (rule leadsTo_Un_duplicate2)
  apply (blast intro: leadsTo_Un_Un wlt_leadsTo
                          [THEN psp2, THEN leadsTo_weaken] leadsTo_refl)
 apply (drule leadsTo_Diff)
 apply (blast intro: subset_imp_leadsTo)
-apply (subgoal_tac "A Int B <= A Int W")
+apply (subgoal_tac "A \<inter> B \<subseteq> A \<inter> W")
  prefer 2
  apply (blast dest!: leadsTo_subset intro!: subset_refl [THEN Int_mono])
 apply (blast intro: leadsTo_Trans subset_imp_leadsTo)
@@ -557,9 +557,9 @@ done
 lemmas completion = completion_lemma [OF refl]
 
 lemma finite_completion_lemma:
-     "finite I ==> (ALL i:I. F : (A i) leadsTo (A' i Un C)) -->   
-                   (ALL i:I. F : (A' i) co (A' i Un C)) -->  
-                   F : (INT i:I. A i) leadsTo ((INT i:I. A' i) Un C)"
+     "finite I ==> (\<forall>i \<in> I. F \<in> (A i) leadsTo (A' i \<union> C)) -->   
+                   (\<forall>i \<in> I. F \<in> (A' i) co (A' i \<union> C)) -->  
+                   F \<in> (\<Inter>i \<in> I. A i) leadsTo ((\<Inter>i \<in> I. A' i) \<union> C)"
 apply (erule finite_induct, auto)
 apply (rule completion)
    prefer 4
@@ -569,15 +569,15 @@ done
 
 lemma finite_completion: 
      "[| finite I;   
-         !!i. i:I ==> F : (A i) leadsTo (A' i Un C);  
-         !!i. i:I ==> F : (A' i) co (A' i Un C) |]    
-      ==> F : (INT i:I. A i) leadsTo ((INT i:I. A' i) Un C)"
+         !!i. i \<in> I ==> F \<in> (A i) leadsTo (A' i \<union> C);  
+         !!i. i \<in> I ==> F \<in> (A' i) co (A' i \<union> C) |]    
+      ==> F \<in> (\<Inter>i \<in> I. A i) leadsTo ((\<Inter>i \<in> I. A' i) \<union> C)"
 by (blast intro: finite_completion_lemma [THEN mp, THEN mp])
 
 lemma stable_completion: 
-     "[| F : A leadsTo A';  F : stable A';    
-         F : B leadsTo B';  F : stable B' |]  
-    ==> F : (A Int B) leadsTo (A' Int B')"
+     "[| F \<in> A leadsTo A';  F \<in> stable A';    
+         F \<in> B leadsTo B';  F \<in> stable B' |]  
+    ==> F \<in> (A \<inter> B) leadsTo (A' \<inter> B')"
 apply (unfold stable_def)
 apply (rule_tac C1 = "{}" in completion [THEN leadsTo_weaken_R])
 apply (force+)
@@ -585,9 +585,9 @@ done
 
 lemma finite_stable_completion: 
      "[| finite I;   
-         !!i. i:I ==> F : (A i) leadsTo (A' i);  
-         !!i. i:I ==> F : stable (A' i) |]    
-      ==> F : (INT i:I. A i) leadsTo (INT i:I. A' i)"
+         !!i. i \<in> I ==> F \<in> (A i) leadsTo (A' i);  
+         !!i. i \<in> I ==> F \<in> stable (A' i) |]    
+      ==> F \<in> (\<Inter>i \<in> I. A i) leadsTo (\<Inter>i \<in> I. A' i)"
 apply (unfold stable_def)
 apply (rule_tac C1 = "{}" in finite_completion [THEN leadsTo_weaken_R])
 apply (simp_all (no_asm_simp))
